wip

src/localdrf/LocalDRF_PF.v
@@ -45,66 +45,275 @@ Proof.
   { eauto. }
 Qed.
 
+Notation "p \\2// q" :=
+  (fun x0 x1 => __guard__(p x0 x1 \/ q x0 x1))
+    (at level 50, no associativity).
+
+Notation "p \\3// q" :=
+  (fun x0 x1 x2 => __guard__(p x0 x1 x2 \/ q x0 x1 x2))
+    (at level 50, no associativity).
+
+Definition lb_time (l: list Time.t) (ts ts': Time.t) :=
+  forall t (IN: List.In t l) (LT: Time.lt ts t),
+    Time.lt ts' t.
+
+Lemma eq_lb_time l ts
+  :
+    lb_time l ts ts.
+Proof.
+  ii. auto.
+Qed.
+
+Lemma lb_time_exists l ts
+  :
+    exists ts', <<TS: Time.lt ts ts'>> /\ <<LB: lb_time l ts ts'>>.
+Proof.
+  induction l.
+  { exists (Time.incr ts). econs; ss.
+    eapply Time.incr_spec. }
+  { des. destruct (Time.le_lt_dec a ts').
+    { destruct (Time.le_lt_dec a ts).
+      { exists ts'. split; ss. ii. ss. des.
+        { subst. exfalso. eapply Time.lt_strorder.
+          eapply (@TimeFacts.le_lt_lt t ts); eauto. }
+        { eauto. }
+      }
+      { exists (Time.middle ts a). split; ss.
+        { eapply Time.middle_spec; eauto. }
+        { ii. ss. des.
+          { subst. eapply Time.middle_spec; eauto. }
+          { exploit LB; eauto. i.
+            transitivity ts'; eauto.
+            eapply TimeFacts.lt_le_lt; eauto.
+            eapply Time.middle_spec; eauto. }
+        }
+      }
+    }
+    { exists ts'. split; ss. ii. ss. des.
+      { subst. auto. }
+      { eapply LB; eauto. }
+    }
+  }
+Qed.
+
+Lemma lb_time_lower l ts ts'0 ts'1
+      (LB: lb_time l ts ts'0)
+      (TS: Time.le ts'1 ts'0)
+  :
+    lb_time l ts ts'1.
+Proof.
+  ii. exploit LB; eauto.
+  i. eapply TimeFacts.le_lt_lt; eauto.
+Qed.
+
+
+Definition memory_times_wf (times: Loc.t -> list Time.t) (mem: Memory.t): Prop :=
+  forall loc to from msg
+         (GET: Memory.get loc to mem = Some (from, msg)),
+    (<<FROM: List.In from (times loc)>>) /\ (<<TO: List.In to (times loc)>>).
+
+Definition memory_times_wf_strong (times: Loc.t -> list Time.t) (mem: Memory.t): Prop :=
+  forall loc to from msg
+         (GET: Memory.get loc to mem = Some (from, msg)),
+    (<<FROM: List.In from (times loc)>>) /\ (<<TO: List.In to (times loc)>>) /\
+    (<<CAP: List.In (Time.incr to) (times loc)>>).
+
+Lemma memory_times_wf_strong_wf
+  :
+    memory_times_wf_strong <2= memory_times_wf.
+Proof.
+  ii. eapply PR in GET. des. auto.
+Qed.
+
+Inductive all_promises (proms: Ident.t -> Loc.t -> Time.t -> Prop): Loc.t -> Time.t -> Prop :=
+| all_promises_intro
+    tid loc ts
+    (PROMS: proms tid loc ts)
+  :
+    all_promises proms loc ts
+.
+Hint Constructors all_promises.
+
+Lemma reserve_future_memory_unch
+      prom0 mem0 prom1 mem1
+      (FUTURE: reserve_future_memory prom0 mem0 prom1 mem1)
+      loc to from msg
+      (GETMEM: Memory.get loc to mem0 = Some (from, msg))
+      (GETPROM: Memory.get loc to prom0 = None)
+  :
+    (<<GETMEM: Memory.get loc to mem1 = Some (from, msg)>>) /\
+    (<<GETPROM: Memory.get loc to prom1 = None>>).
+Proof.
+  ginduction FUTURE; eauto. i. inv HD; clarify.
+  { eapply IHFUTURE; eauto.
+    - erewrite Memory.add_o; eauto. des_ifs.
+      ss. des; clarify.
+      eapply Memory.add_get0 in MEM. des. clarify.
+    - erewrite Memory.add_o; eauto. des_ifs.
+      ss. des; clarify.
+      eapply Memory.add_get0 in MEM. des. clarify. }
+  { apply split_succeed_wf in PROMISES. des. clarify. }
+  { apply lower_succeed_wf in PROMISES. des. clarify. inv MSG_LE. }
+  { eapply IHFUTURE; eauto.
+    - erewrite Memory.remove_o; eauto. des_ifs.
+      ss. des; clarify.
+      eapply Memory.remove_get0 in PROMISES. des. clarify.
+    - erewrite Memory.remove_o; eauto. des_ifs. }
+Qed.
+
+Lemma memory_get_disjoint_strong mem loc from0 to0 from1 to1 msg0 msg1
+      (GET0: Memory.get loc to0 mem = Some (from0, msg0))
+      (GET1: Memory.get loc to1 mem = Some (from1, msg1))
+  :
+    (to0 = to1 /\ from0 = from1 /\ msg0 = msg1) \/
+    (<<TS: Time.le to0 from1>> /\ <<TS: Time.lt to0 to1>>) \/
+    (<<TS: Time.le to1 from0>> /\ <<TS: Time.lt to1 to0>>).
+Proof.
+  destruct (Time.le_lt_dec to0 to1).
+  { destruct l.
+    { dup H. eapply memory_get_from_mon in H; eauto. }
+    { inv H. clarify. auto. }
+  }
+  { dup l. eapply memory_get_from_mon in l; eauto. }
+Qed.
+
+
+Inductive reserving_tevent: forall (e: ThreadEvent.t), Prop :=
+| reserving_tevent_reserve
+    loc from to kind
+  :
+    reserving_tevent (ThreadEvent.promise loc from to Message.reserve kind)
+.
+Hint Constructors reserving_tevent.
+
+Definition reserving_trace (lang: language) (tr: Trace.t lang): Prop :=
+  List.Forall (fun the => reserving_tevent (snd the)) tr.
+
+Lemma reserve_future_memory_steps
+      lang st vw sc prom0 mem0 prom1 mem1
+      (FUTURE: reserve_future_memory prom0 mem0 prom1 mem1)
+  :
+    exists tr,
+      (<<STEPS: Trace.steps tr
+                            (Thread.mk lang st (Local.mk vw prom0) sc mem0)
+                            (Thread.mk lang st (Local.mk vw prom1) sc mem1)>>) /\
+      (<<RESERVING: reserving_trace tr>>)
+.
+Proof.
+  ginduction FUTURE.
+  { i. exists []. splits; eauto. econs; eauto. }
+  { i. exploit IHFUTURE; eauto. i. des. esplits.
+    { eapply Trace.steps_trans; [|apply STEPS|ss].
+      econs 1. econs; eauto. }
+    { econs; ss. }
+  }
+Qed.
+
+Lemma reserve_future_memory_unchangable
+      prom0 mem0 prom1 mem1 loc to from msg
+      (FUTURE: reserve_future_memory prom0 mem0 prom1 mem1)
+      (UNCH: unchangable mem0 prom0 loc to from msg)
+  :
+    unchangable mem1 prom1 loc to from msg.
+Proof.
+  ginduction FUTURE; eauto. i. exploit IHFUTURE; eauto.
+  eapply unchangable_promise; eauto.
+Qed.
+
+Lemma reserve_future_memory_future
+      vw sc prom0 mem0 prom1 mem1
+      (LOCAL: Local.wf (Local.mk vw prom0) mem0)
+      (SC: Memory.closed_timemap sc mem0)
+      (MEM: Memory.closed mem0)
+      (FUTURE: reserve_future_memory prom0 mem0 prom1 mem1)
+  :
+    (<<LOCAL: Local.wf (Local.mk vw prom1) mem1>>) /\
+    (<<SC: Memory.closed_timemap sc mem1>>) /\
+    (<<MEM: Memory.closed mem1>>).
+Proof.
+  ginduction FUTURE; eauto. i.
+  exploit Local.promise_step_future.
+  { econs.
+    - instantiate (9:=Local.mk vw prom0). eauto.
+    - eauto.
+    - eauto. }
+  all: eauto. i. des. ss. eapply IHFUTURE; eauto.
+Qed.
+
+Lemma reserve_future_concrete_same_promise2 prom0 mem0 prom1 mem1 loc from to val released
+      (FUTURE: reserve_future_memory prom0 mem0 prom1 mem1)
+      (GET: Memory.get loc to prom1 = Some (from, Message.concrete val released))
+  :
+    Memory.get loc to prom0 = Some (from, Message.concrete val released).
+Proof.
+  ginduction FUTURE; auto. i. apply IHFUTURE in GET; auto.
+  inv HD; des; clarify.
+  - erewrite Memory.add_o in GET; eauto. des_ifs.
+  - erewrite Memory.lower_o in GET; eauto. des_ifs.
+  - erewrite Memory.remove_o in GET; eauto. des_ifs.
+Qed.
+
+Lemma reserve_future_read_commute
+      vw0 prom0 mem0 loc to val released ord vw1 prom' prom1 mem1
+      (READ: Local.read_step (Local.mk vw0 prom0) mem0 loc to val released ord (Local.mk vw1 prom'))
+      (FUTURE: reserve_future_memory prom0 mem0 prom1 mem1)
+  :
+    Local.read_step (Local.mk vw0 prom1) mem1 loc to val released ord (Local.mk vw1 prom1).
+Proof.
+  inv READ. clarify. econs; eauto.
+  eapply reserve_future_concrete_same; eauto.
+Qed.
+
+Lemma joined_view_semi_closed
+      views view mem loc ts
+      (MEM: List.Forall (fun vw => semi_closed_view vw mem loc ts) views)
+      (JOINED: joined_view views view)
+      (INHABITED: Memory.inhabited mem)
+  :
+    semi_closed_view view mem loc ts.
+Proof.
+  ginduction JOINED; eauto.
+  - i. eapply closed_view_semi_closed. apply Memory.closed_view_bot. auto.
+  - i. eapply semi_closed_view_join; eauto.
+    eapply List.Forall_forall in VIEW; [|eauto]. ss.
+Qed.
+
+Lemma traces_steps_future
+      lang tr e1 e2
+      (STEPS: @Trace.steps lang tr e1 e2)
+      (WF1: Local.wf e1.(Thread.local) e1.(Thread.memory))
+      (SC1: Memory.closed_timemap e1.(Thread.sc) e1.(Thread.memory))
+      (CLOSED1: Memory.closed e1.(Thread.memory)):
+  (<<WF2: Local.wf e2.(Thread.local) e2.(Thread.memory)>>) /\
+  (<<SC2: Memory.closed_timemap e2.(Thread.sc) e2.(Thread.memory)>>) /\
+  (<<CLOSED2: Memory.closed e2.(Thread.memory)>>) /\
+  (<<TVIEW_FUTURE: TView.le e1.(Thread.local).(Local.tview) e2.(Thread.local).(Local.tview)>>) /\
+  (<<SC_FUTURE: TimeMap.le e1.(Thread.sc) e2.(Thread.sc)>>) /\
+  (<<MEM_FUTURE: Memory.future e1.(Thread.memory) e2.(Thread.memory)>>)
+.
+Proof.
+  ginduction STEPS.
+  - i. splits; auto.
+    + refl.
+    + refl.
+  - i. exploit Thread.step_future; eauto. i. des.
+    exploit IHSTEPS; eauto. i. des. splits; auto.
+    + etrans; eauto.
+    + etrans; eauto.
+    + etrans; eauto.
+Qed.
+
+
+
+
 
 Section SIM.
 
   Variable L: Loc.t -> bool.
   Variable times: Loc.t -> list Time.t.
 
-  Definition lb_time (l: list Time.t) (ts ts': Time.t) :=
-    forall t (IN: List.In t l) (LT: Time.lt ts t),
-      Time.lt ts' t.
 
-  Lemma eq_lb_time l ts
-    :
-      lb_time l ts ts.
-  Proof.
-    ii. auto.
-  Qed.
-
-  Lemma lb_time_exists l ts
-    :
-      exists ts', <<TS: Time.lt ts ts'>> /\ <<LB: lb_time l ts ts'>>.
-  Proof.
-    induction l.
-    { exists (Time.incr ts). econs; ss.
-      eapply Time.incr_spec. }
-    { des. destruct (Time.le_lt_dec a ts').
-      { destruct (Time.le_lt_dec a ts).
-        { exists ts'. split; ss. ii. ss. des.
-          { subst. exfalso. eapply Time.lt_strorder.
-            eapply (@TimeFacts.le_lt_lt t ts); eauto. }
-          { eauto. }
-        }
-        { exists (Time.middle ts a). split; ss.
-          { eapply Time.middle_spec; eauto. }
-          { ii. ss. des.
-            { subst. eapply Time.middle_spec; eauto. }
-            { exploit LB; eauto. i.
-              transitivity ts'; eauto.
-              eapply TimeFacts.lt_le_lt; eauto.
-              eapply Time.middle_spec; eauto. }
-          }
-        }
-      }
-      { exists ts'. split; ss. ii. ss. des.
-        { subst. auto. }
-        { eapply LB; eauto. }
-      }
-    }
-  Qed.
-
-  Lemma lb_time_lower l ts ts'0 ts'1
-        (LB: lb_time l ts ts'0)
-        (TS: Time.le ts'1 ts'0)
-    :
-      lb_time l ts ts'1.
-  Proof.
-    ii. exploit LB; eauto.
-    i. eapply TimeFacts.le_lt_lt; eauto.
-  Qed.
-
-
+  (* sim memory *)
 
   Inductive sim_memory_content
             (F: Prop)
@@ -144,37 +353,6 @@ Section SIM.
   .
   Hint Constructors sim_memory_content.
 
-  (* Record sim_memory (forgets: Loc.t -> Time.t -> option Time.t -> Prop) *)
-  (*        (mem_src mem_tgt: Memory.t) : Prop := *)
-  (*   { *)
-  (*     sim_memory_forgets_wf: *)
-  (*       forall loc ts ts' *)
-  (*              (FORGET: forgets loc ts (Some ts')), *)
-  (*         (<<LB: lb_time (times loc) ts ts'>>) /\ *)
-  (*         (<<LOC: L loc>>) /\ *)
-  (*         (<<TS: Time.lt ts ts'>>); *)
-  (*     sim_memory_forgets_message: *)
-  (*       forall loc ts ts' *)
-  (*              (FORGET: forgets loc ts ts'), *)
-  (*       exists from val released, *)
-  (*         (<<GET: Memory.get loc ts mem_tgt = Some (from, Message.concrete val released)>>); *)
-  (*     sim_memory_normal: *)
-  (*       forall loc ts (NLOC: L loc), Memory.get loc ts mem_src = Memory.get loc ts mem_tgt; *)
-  (*     sim_memory_get: *)
-  (*       forall loc ts val released *)
-  (*              (LOC: L loc) *)
-  (*              (NORMAL: forall ts', ~ forgets loc ts ts'), *)
-  (*         (exists from, <<GET: Memory.get loc ts mem_src = Some (from, Message.concrete val released)>>) *)
-  (*         <-> *)
-  (*         (exists from, <<GET: Memory.get loc ts mem_tgt = Some (from, Message.concrete val released)>>); *)
-  (*     sim_memory_covered: *)
-  (*       forall loc ts (COVER: covered loc ts mem_src) (LOC: L loc), *)
-  (*         (<<COVER: covered loc ts mem_tgt>>) \/ *)
-  (*         (exists from to, *)
-  (*             (<<FORGET: forgets loc to (Some from)>>) /\ *)
-  (*             (<<ITV: Interval.mem (from, to) ts>>)); *)
-  (*   }. *)
-
   Record sim_memory
          (F: Loc.t -> Time.t -> Prop)
          (extra: Loc.t -> Time.t -> Time.t -> Prop)
@@ -192,168 +370,6 @@ Section SIM.
           (<<UNIQUE: forall from' (EXTRA: extra loc ts from'),
               from' = from>>);
     }.
-
-  Inductive sim_promise_content
-            (F: Prop)
-            (extra: Time.t -> Prop)
-            (loc: Loc.t) (ts: Time.t)
-    :
-      option (Time.t * Message.t) -> option (Time.t * Message.t) -> Prop :=
-  | sim_promise_content_none
-      (NPROM: ~ F)
-      (NEXTRA: forall t, ~ extra t)
-      (NLOC: L loc)
-    :
-      sim_promise_content F extra loc ts None None
-  | sim_promise_content_normal
-      (NPROM: ~ F)
-      (NEXTRA: forall t, ~ extra t)
-      (NLOC: ~ L loc)
-      cnt
-    :
-      sim_promise_content F extra loc ts cnt cnt
-  | sim_promise_content_reserve
-      (NPROM: ~ F)
-      (NEXTRA: forall t, ~ extra t)
-      (LOC: L loc)
-      from_src from_tgt
-    :
-      sim_promise_content F extra loc ts
-                          (Some (from_src, Message.reserve))
-                          (Some (from_tgt, Message.reserve))
-  | sim_promise_content_forget
-      (PROM: F)
-      (NEXTRA: forall t, ~ extra t)
-      (LOC: L loc)
-      from_src from_tgt val released
-    :
-      sim_promise_content F extra loc ts
-                          (Some (from_src, Message.reserve))
-                          (Some (from_tgt, Message.concrete val released))
-  | sim_promise_content_extra
-      from
-      (NPROM: ~ F)
-      (LOC: L loc)
-      (EXTRA: extra from)
-    :
-      sim_promise_content F extra loc ts (Some (from, Message.reserve)) None
-  .
-  Hint Constructors sim_promise_content.
-
-  Record sim_promise
-         (self: Loc.t -> Time.t -> Prop)
-         (extra: Loc.t -> Time.t -> Time.t -> Prop)
-         (prom_src prom_tgt: Memory.t): Prop :=
-    {
-      sim_promise_contents:
-        forall loc ts,
-          sim_promise_content (self loc ts) (extra loc ts)
-                              loc ts
-                              (Memory.get loc ts prom_src)
-                              (Memory.get loc ts prom_tgt);
-      sim_promise_wf:
-        forall loc from ts (EXTRA: extra loc ts from),
-          (<<FORGET: self loc from>>) /\
-          (<<LB: lb_time (times loc) from ts>>) /\
-          (<<TS: Time.lt from ts>>);
-      sim_promise_extra:
-        forall loc ts (SELF: self loc ts),
-        exists to,
-          (<<GET: Memory.get loc to prom_src = Some (ts, Message.reserve)>>) /\
-          (<<TS: Time.lt ts to>>);
-    }.
-
-  Inductive sim_local
-            (self: Loc.t -> Time.t -> Prop)
-            (extra: Loc.t -> Time.t -> Time.t -> Prop)
-    :
-      forall (lc_src lc_tgt: Local.t), Prop :=
-  | sim_local_intro
-      tvw prom_src prom_tgt
-      (PROMS: sim_promise self extra prom_src prom_tgt)
-    :
-      sim_local self extra (Local.mk tvw prom_src) (Local.mk tvw prom_tgt)
-  .
-  Hint Constructors sim_local.
-
-  Inductive sim_statelocal
-            (self: Loc.t -> Time.t -> Prop)
-            (extra: Loc.t -> Time.t -> Time.t -> Prop)
-    :
-      sigT (@Language.state ProgramEvent.t) * Local.t -> sigT (@Language.state ProgramEvent.t) * Local.t -> Prop :=
-  | forget_statelocal_intro
-      st lc_src lc_tgt
-      (LOCAL: sim_local self extra lc_src lc_tgt)
-    :
-      sim_statelocal self extra (st, lc_src) (st, lc_tgt)
-  .
-
-  Inductive all_promises (proms: Ident.t -> Loc.t -> Time.t -> Prop): Loc.t -> Time.t -> Prop :=
-  | all_promises_intro
-      tid loc ts
-      (PROMS: proms tid loc ts)
-    :
-      all_promises proms loc ts
-  .
-  Hint Constructors all_promises.
-
-  Lemma sim_read_step F extra self lc_src lc_tgt mem_src mem_tgt loc to val released ord
-        lc_tgt'
-        (STEPTGT: Local.read_step lc_tgt mem_tgt loc to val released ord lc_tgt')
-        (NOREAD: ~ F loc to)
-        (MEM: sim_memory F extra mem_src mem_tgt)
-        (LOCAL: sim_local self extra lc_src lc_tgt)
-    :
-      exists lc_src',
-        (<<STEPSRC: Local.read_step lc_src mem_src loc to val released ord lc_src'>>) /\
-        (<<SIM: sim_local self extra lc_src' lc_tgt'>>) /\
-        (<<GETSRC: exists from, Memory.get loc to mem_src = Some (from, Message.concrete val released)>>) /\
-        (<<GETTGT: exists from, Memory.get loc to mem_tgt = Some (from, Message.concrete val released)>>)
-  .
-  Proof.
-    inv LOCAL. inv STEPTGT.
-    set (MEM0:= MEM.(sim_memory_contents) loc to). rewrite GET in *. inv MEM0; ss.
-    esplits; eauto.
-  Qed.
-
-  Lemma sim_fence_step self extra lc_src lc_tgt sc ordr ordw
-        sc' lc_tgt'
-        (STEPTGT: Local.fence_step lc_tgt sc ordr ordw lc_tgt' sc')
-        (LOCAL: sim_local self extra lc_src lc_tgt)
-    :
-      exists lc_src',
-        (<<STEPSRC: Local.fence_step lc_src sc ordr ordw lc_src' sc'>>) /\
-        (<<SIM: sim_local self extra lc_src' lc_tgt'>>)
-  .
-  Proof.
-    inv LOCAL. inv STEPTGT. esplits.
-    - econs; ss; eauto. ii.
-      set (PROM:= PROMS.(sim_promise_contents) loc t).
-      rewrite GET in *. inv PROM; ss.
-      exploit RELEASE; eauto.
-    - econs; ss; eauto.
-  Qed.
-
-  Lemma sim_promise_consistent self extra lc_src lc_tgt
-        (CONSISTENT: Local.promise_consistent lc_tgt)
-        (SIM: sim_local self extra lc_src lc_tgt)
-    :
-      Local.promise_consistent lc_src.
-  Proof.
-    inv SIM. ii. ss.
-    set (PROM:= PROMS.(sim_promise_contents) loc ts).
-    rewrite PROMISE in *. inv PROM. eauto.
-  Qed.
-
-  Lemma sim_failure_step self extra lc_src lc_tgt
-        (STEPTGT: Local.failure_step lc_tgt)
-        (SIM: sim_local self extra lc_src lc_tgt)
-    :
-      Local.failure_step lc_src.
-  Proof.
-    inv STEPTGT. econs.
-    eapply sim_promise_consistent; eauto.
-  Qed.
 
   Lemma sim_memory_others_self_wf
         F extra mem_src mem_tgt
@@ -374,469 +390,6 @@ Section SIM.
     inv MEMORY0; clarify; (exfalso; eapply NEXTRA; eauto).
   Qed.
 
-  Notation "p \\2// q" :=
-    (fun x0 x1 => __guard__(p x0 x1 \/ q x0 x1))
-      (at level 50, no associativity).
-
-  Notation "p \\3// q" :=
-    (fun x0 x1 x2 => __guard__(p x0 x1 x2 \/ q x0 x1 x2))
-      (at level 50, no associativity).
-
-  Lemma sim_promise_step_normal others self extra_others extra_self
-        mem_src mem_tgt prom_src prom_tgt
-        loc from to msg prom_tgt' mem_tgt' kind
-        (NLOC: ~ L loc)
-        (STEPTGT: Memory.promise prom_tgt mem_tgt loc from to msg prom_tgt' mem_tgt' kind)
-        (MEM: sim_memory (others \\2// self) (extra_others \\3// extra_self) mem_src mem_tgt)
-        (MEMSRC: Memory.closed mem_src)
-        (MEMTGT: Memory.closed mem_tgt)
-        (WFSRC: Memory.le prom_src mem_src)
-        (WFTGT: Memory.le prom_tgt mem_tgt)
-        (PROMISE: sim_promise self extra_self prom_src prom_tgt)
-        (SEMI: semi_closed_message msg mem_src loc to)
-    :
-      exists prom_src' mem_src',
-        (<<STEPSRC: Memory.promise prom_src mem_src loc from to msg prom_src' mem_src' kind>>) /\
-        (<<MEM: sim_memory (others \\2// self) (extra_others \\3// extra_self) mem_src' mem_tgt'>>) /\
-        (<<PROMISE: sim_promise self extra_self prom_src' prom_tgt'>>) /\
-        (<<CLOSED: Memory.closed_message msg mem_src'>>)
-  .
-  Proof.
-    generalize (sim_memory_others_self_wf MEM). intros PROMSWF.
-    generalize (sim_memory_extra_others_self_wf MEM). intros EXTRAWF.
-    inv STEPTGT.
-
-    (* add case *)
-    - exploit add_succeed_wf; try apply MEM0. i. des.
-      hexploit (@Memory.add_exists mem_src loc from to msg); ss.
-      { i. set (MEM1:= MEM.(sim_memory_contents) loc to2).
-        rewrite GET2 in *. inv MEM1; cycle 1.
-        { exfalso. apply NLOC. des; eauto. }
-        { exfalso. apply NLOC. des; eauto. }
-        ii. eapply DISJOINT; eauto.
-        inv RHS. econs; ss. eapply TimeFacts.le_lt_lt; eauto. }
-      intros [mem_src' ADDMEMSRC].
-      exploit Memory.add_exists_le; try apply ADDMEMSRC; eauto.
-      intros [prom_src' ADDPROMSRC].
-
-      assert (PROMISESRC: Memory.promise prom_src mem_src loc from to msg prom_src' mem_src' Memory.op_kind_add).
-      { econs; eauto. i. subst.
-        set (MEM1:= MEM.(sim_memory_contents) loc to'). rewrite GET in MEM1. inv MEM1; ss.
-        eapply ATTACH; eauto. erewrite NLOC0; eauto. }
-
-      assert (CLOSEDMSG: Memory.closed_message msg mem_src').
-      { destruct msg; auto.
-        eapply semi_closed_message_add; eauto. }
-
-      exists prom_src', mem_src'. splits; auto.
-      + econs.
-        { ii. set (MEM1:= MEM.(sim_memory_contents) loc0 ts).
-          erewrite (@Memory.add_o mem_src'); eauto.
-          erewrite (@Memory.add_o mem_tgt'); eauto.
-          des_ifs; try by (ss; des; clarify).
-          * econs; eauto.
-            { ii. ss. des; clarify; eauto. }
-            { ii. ss. des; clarify; eauto. }
-            { refl. }
-            { i. ss. }
-        }
-        { eapply MEM.(sim_memory_wf); eauto. }
-      + econs.
-        { ii. set (PROM:= PROMISE.(sim_promise_contents) loc0 ts).
-          erewrite (@Memory.add_o prom_src'); eauto.
-          erewrite (@Memory.add_o prom_tgt'); eauto. des_ifs.
-          ss. des; clarify. econs; eauto.
-          { ii. eapply NLOC. eapply PROMSWF; ss. right. eauto. }
-          { ii. eapply NLOC. eapply EXTRAWF; ss. right. eauto. }
-        }
-        { apply PROMISE. }
-        { i. hexploit PROMISE.(sim_promise_extra); eauto. i. des.
-          esplits; eauto. erewrite (@Memory.add_o prom_src'); eauto.
-          des_ifs. ss. des; clarify.
-          exfalso. eapply NLOC. eapply PROMSWF; eauto. right. eauto. }
-
-    (* split case *)
-    - exploit split_succeed_wf; try apply PROMISES. i. des. clarify.
-      set (PROMISE0:= PROMISE.(sim_promise_contents) loc ts3). rewrite GET2 in *.
-      inv PROMISE0; ss.
-      hexploit (@Memory.split_exists prom_src loc from to ts3 (Message.concrete val' released')); ss.
-      { eauto. }
-      intros [prom_src' SPLITPROMSRC].
-      exploit Memory.split_exists_le; try apply SPLITPROMSRC; eauto.
-      intros [mem_src' SPLITMEMSRC].
-
-      assert (PROMISESRC: Memory.promise prom_src mem_src loc from to (Message.concrete val' released') prom_src' mem_src' (Memory.op_kind_split ts3 msg3)).
-      { econs; eauto. }
-
-      assert (CLOSEDMSG: Memory.closed_message (Message.concrete val' released') mem_src').
-      { eapply semi_closed_message_split; eauto. }
-
-      exists prom_src', mem_src'. splits; auto.
-      + econs.
-        { ii. set (MEM1:=MEM.(sim_memory_contents) loc0 ts).
-          erewrite (@Memory.split_o mem_src'); eauto.
-          erewrite (@Memory.split_o mem_tgt'); eauto.
-          des_ifs; try by (ss; des; clarify).
-          { ss. des; clarify. econs; eauto.
-            * refl.
-            * i. ss. }
-          { guardH o. ss. des; clarify. econs; eauto.
-            * refl.
-            * i. ss. }
-        }
-        { apply MEM.(sim_memory_wf); eauto. }
-      + econs.
-        { ii. set (PROM:= PROMISE.(sim_promise_contents) loc0 ts).
-          erewrite (@Memory.split_o prom_src'); eauto.
-          erewrite (@Memory.split_o prom_tgt'); eauto. des_ifs.
-          * ss. des; clarify. econs; eauto.
-            { ii. eapply NLOC. eapply PROMSWF. right. eauto. }
-            { ii. eapply NLOC. eapply EXTRAWF. right. eauto. }
-          * guardH o. ss. des; clarify. econs; eauto. }
-        { apply PROMISE. }
-        { i. hexploit PROMISE.(sim_promise_extra); eauto. i. des.
-          esplits; eauto. erewrite (@Memory.split_o prom_src'); eauto. des_ifs.
-          - ss. des; clarify. exfalso. eapply NLOC. eapply PROMSWF; eauto. right. eauto.
-          - ss. des; clarify. exfalso. eapply NLOC. eapply PROMSWF; eauto. right. eauto. }
-
-    (* lower case *)
-    - exploit lower_succeed_wf; try apply PROMISES. i. des. clarify.
-      set (PROMISE0:= PROMISE.(sim_promise_contents) loc to). rewrite GET in *. inv PROMISE0; ss.
-
-      hexploit (@Memory.lower_exists prom_src loc from to (Message.concrete val released) msg); ss.
-
-      intros [prom_src' LOWERPROMSRC].
-      exploit Memory.lower_exists_le; try apply LOWERPROMSRC; eauto.
-      intros [mem_src' LOWERMEMSRC].
-
-      assert (PROMISESRC: Memory.promise prom_src mem_src loc from to msg prom_src' mem_src' (Memory.op_kind_lower (Message.concrete val released))).
-      { econs; eauto. }
-
-      assert (CLOSEDMSG: Memory.closed_message msg mem_src').
-      { destruct msg; auto.
-        eapply semi_closed_message_lower; eauto. }
-
-      exists prom_src', mem_src'. splits; auto.
-      + econs.
-        { ii. set (MEM1:=MEM.(sim_memory_contents) loc0 ts).
-          erewrite (@Memory.lower_o mem_src'); eauto.
-          erewrite (@Memory.lower_o mem_tgt'); eauto. des_ifs.
-          ss. des; clarify. econs; eauto.
-          * refl.
-          * i. ss. }
-        { apply MEM.(sim_memory_wf); eauto. }
-      + econs.
-        { ii. set (PROM:= PROMISE.(sim_promise_contents) loc0 ts).
-          erewrite (@Memory.lower_o prom_src'); eauto.
-          erewrite (@Memory.lower_o prom_tgt'); eauto. des_ifs.
-          ss. des; clarify. econs; eauto. }
-        { apply PROMISE. }
-        { i. hexploit PROMISE.(sim_promise_extra); eauto. i. des.
-          esplits; eauto. erewrite (@Memory.lower_o prom_src'); eauto. des_ifs.
-          ss. des; clarify. }
-
-    (* cancel case *)
-    - exploit Memory.remove_get0; try apply PROMISES. i. des.
-      set (PROMISE0 := PROMISE.(sim_promise_contents) loc to). rewrite GET in *.
-      inv PROMISE0; ss.
-
-      hexploit (@Memory.remove_exists prom_src loc from to Message.reserve); ss.
-      intros [prom_src' REMOVEPROMSRC].
-      exploit Memory.remove_exists_le; try apply REMOVEPROMSRC; eauto.
-      intros [mem_src' REMOVEMEMSRC].
-
-      assert (PROMISESRC: Memory.promise prom_src mem_src loc from to Message.reserve prom_src' mem_src' Memory.op_kind_cancel).
-      { econs; eauto. }
-
-      exists prom_src', mem_src'.
-      splits; auto.
-      + econs.
-        { ii. set (MEM1:=MEM.(sim_memory_contents) loc0 ts).
-          erewrite (@Memory.remove_o mem_src'); eauto.
-          erewrite (@Memory.remove_o mem_tgt'); eauto.
-          des_ifs; try by (des; ss; clarify).
-          * ss. des; clarify. econs; eauto. }
-        { apply MEM. }
-      + econs.
-        { ii. set (PROM:= PROMISE.(sim_promise_contents) loc0 ts).
-          erewrite (@Memory.remove_o prom_src'); eauto.
-          erewrite (@Memory.remove_o prom_tgt'); eauto. des_ifs.
-          ss. des; clarify. econs 2; eauto. }
-        { apply PROMISE. }
-        { i. hexploit PROMISE.(sim_promise_extra); eauto. i. des.
-          esplits; eauto. erewrite (@Memory.remove_o prom_src'); eauto. des_ifs.
-          ss. des; clarify. exfalso. eapply NLOC. eapply PROMSWF; eauto. right. eauto. }
-  Qed.
-
-  Lemma sim_write_step_normal
-        others self extra_others extra_self lc_src lc_tgt sc mem_src mem_tgt
-        lc_tgt' sc' mem_tgt' loc from to val ord releasedm released kind
-        (NLOC: ~ L loc)
-        (STEPTGT: Local.write_step lc_tgt sc mem_tgt loc from to val releasedm released ord lc_tgt' sc' mem_tgt' kind)
-        (MEM: sim_memory (others \\2// self) (extra_others \\3// extra_self) mem_src mem_tgt)
-        (SCSRC: Memory.closed_timemap sc mem_src)
-        (SCTGT: Memory.closed_timemap sc mem_tgt)
-        (MEMSRC: Memory.closed mem_src)
-        (MEMTGT: Memory.closed mem_tgt)
-        (LOCALSRC: Local.wf lc_src mem_src)
-        (LOCALTGT: Local.wf lc_tgt mem_tgt)
-        (SIM: sim_local self extra_self lc_src lc_tgt)
-
-        (RELEASEDMCLOSED: Memory.closed_opt_view releasedm mem_src)
-        (RELEASEDMWF: View.opt_wf releasedm)
-    :
-      exists lc_src' mem_src',
-        (<<STEPSRC: Local.write_step lc_src sc mem_src loc from to val releasedm released ord lc_src' sc' mem_src' kind>>) /\
-        (<<MEM: sim_memory (others \\2// self) (extra_others \\3// extra_self) mem_src' mem_tgt'>>) /\
-        (<<SIM: sim_local self extra_self lc_src' lc_tgt'>>)
-  .
-  Proof.
-    inv STEPTGT. inv WRITE. inv SIM. inv LOCALSRC. inv LOCALTGT.
-
-    hexploit sim_promise_step_normal; eauto.
-    { ss. econs. unfold TView.write_released. des_ifs; econs.
-      eapply semi_closed_view_join.
-      - inv MEMSRC. eapply unwrap_closed_opt_view; auto.
-        eapply closed_opt_view_semi_closed. auto.
-      - ss. setoid_rewrite LocFun.add_spec_eq. des_ifs.
-        + eapply semi_closed_view_join.
-          * eapply closed_view_semi_closed. inv TVIEW_CLOSED. auto.
-          * inv MEMSRC. eapply semi_closed_view_singleton. auto.
-        + eapply semi_closed_view_join.
-          * eapply closed_view_semi_closed. inv TVIEW_CLOSED. auto.
-          * inv MEMSRC. eapply semi_closed_view_singleton. auto.
-    }
-    i. des. ss.
-
-    hexploit (@Memory.remove_exists
-                prom_src' loc from to
-                (Message.concrete val (TView.write_released tvw sc loc to releasedm ord))).
-    { set (PROM:= PROMISE0.(sim_promise_contents) loc to).
-      eapply Memory.remove_get0 in REMOVE. des.
-      rewrite GET in *. inv PROM; ss. }
-    intros [prom_src'' REMOVESRC].
-
-    assert (NSELF: forall ts, ~ self loc ts).
-    { ii. set (PROM:= PROMISE0.(sim_promise_contents) loc to). inv PROM; ss.
-      eapply NLOC. eapply sim_memory_others_self_wf; eauto. ss. right. eauto. }
-
-    esplits; eauto.
-
-    - econs; ss.
-      + econs; eauto.
-      + ii. set (PROM:=PROMS.(sim_promise_contents) loc t).
-        rewrite GET in *. inv PROM; ss.
-        exploit RELEASE; eauto.
-
-    - econs; auto. econs.
-      { ii. set (PROM:=PROMISE0.(sim_promise_contents) loc0 ts).
-        erewrite (@Memory.remove_o prom_src''); eauto.
-        erewrite (@Memory.remove_o promises2); eauto. des_ifs.
-        ss. des; subst. econs 2; eauto.
-        ii. exploit sim_memory_extra_others_self_wf.
-        { eapply MEM0. }
-        { right. eauto. }
-        { ii. ss. }
-      }
-      { apply PROMISE0. }
-      { i. set (PROM:=PROMISE0.(sim_promise_extra) loc0 ts SELF). des.
-        esplits; eauto. erewrite (@Memory.remove_o prom_src''); eauto.
-        des_ifs. ss. des; clarify. exfalso. eapply NSELF; eauto. }
-  Qed.
-
-
-  Inductive sim_promise_content_strong
-            (F: Prop)
-            (extra: Time.t -> Prop)
-            (extra_all: Time.t -> Time.t -> Prop)
-            (loc: Loc.t) (ts: Time.t)
-    :
-      option (Time.t * Message.t) -> option (Time.t * Message.t) -> Prop :=
-  | sim_promise_content_strong_none
-      (NPROM: ~ F)
-      (NEXTRA: forall t, ~ extra t)
-      (NLOC: L loc)
-    :
-      sim_promise_content_strong F extra extra_all loc ts None None
-  | sim_promise_content_strong_normal
-      (NPROM: ~ F)
-      (NEXTRA: forall t, ~ extra t)
-      (NLOC: ~ L loc)
-      cnt
-    :
-      sim_promise_content_strong F extra extra_all loc ts cnt cnt
-  | sim_promise_content_strong_reserve
-      (NPROM: ~ F)
-      (NEXTRA: forall t, ~ extra t)
-      (LOC: L loc)
-      from_src from_tgt
-      (EXTRA: from_tgt = from_src \/ extra_all from_src from_tgt)
-    :
-      sim_promise_content_strong F extra extra_all loc ts
-                          (Some (from_src, Message.reserve))
-                          (Some (from_tgt, Message.reserve))
-  | sim_promise_content_strong_forget
-      (PROM: F)
-      (NEXTRA: forall t, ~ extra t)
-      (LOC: L loc)
-      from_src from_tgt val released
-      (EXTRA: from_tgt = from_src \/ extra_all from_src from_tgt)
-    :
-      sim_promise_content_strong F extra extra_all loc ts
-                          (Some (from_src, Message.reserve))
-                          (Some (from_tgt, Message.concrete val released))
-  | sim_promise_content_strong_extra
-      from
-      (NPROM: ~ F)
-      (LOC: L loc)
-      (EXTRA: extra from)
-    :
-      sim_promise_content_strong F extra extra_all loc ts (Some (from, Message.reserve)) None
-  .
-  Hint Constructors sim_promise_content_strong.
-
-
-  Lemma sim_promise_content_strong_sim_promise_content
-        loc ts F extra get0 get1 extra_all
-        (SIM: sim_promise_content_strong F extra extra_all loc ts  get0 get1)
-    :
-      sim_promise_content F extra loc ts get0 get1.
-  Proof.
-    inv SIM; econs; eauto.
-  Qed.
-
-  Record sim_promise_strong
-         (self: Loc.t -> Time.t -> Prop)
-         (extra: Loc.t -> Time.t -> Time.t -> Prop)
-         (extra_all: Loc.t -> Time.t -> Time.t -> Prop)
-         (prom_src prom_tgt: Memory.t): Prop :=
-    {
-      sim_promise_strong_contents:
-        forall loc ts,
-          sim_promise_content_strong (self loc ts) (extra loc ts) (extra_all loc)
-                                     loc ts
-                                     (Memory.get loc ts prom_src)
-                                     (Memory.get loc ts prom_tgt);
-      sim_promise_strong_wf:
-        forall loc from ts (EXTRA: extra loc ts from),
-          (<<FORGET: self loc from>>) /\
-          (<<LB: lb_time (times loc) from ts>>) /\
-          (<<TS: Time.lt from ts>>);
-      sim_promise_strong_extra:
-        forall loc ts (SELF: self loc ts),
-        exists to,
-          (<<GET: Memory.get loc to prom_src = Some (ts, Message.reserve)>>) /\
-          (<<TS: Time.lt ts to>>);
-    }.
-
-  Lemma sim_promise_strong_sim_promise
-        self extra extra_all prom_src prom_tgt
-        (SIM: sim_promise_strong self extra extra_all prom_src prom_tgt)
-    :
-      sim_promise self extra prom_src prom_tgt.
-  Proof.
-    econs.
-    - ii. eapply sim_promise_content_strong_sim_promise_content; eauto.
-      eapply SIM; eauto.
-    - apply SIM.
-    - apply SIM.
-  Qed.
-
-  Record sim_promise_list
-         (self: Loc.t -> Time.t -> Prop)
-         (extra: Loc.t -> Time.t -> Time.t -> Prop)
-         (extra_all: Loc.t -> Time.t -> Time.t -> Prop)
-         (prom_src prom_tgt: Memory.t)
-         (l: list (Loc.t * Time.t)): Prop :=
-    {
-      sim_promise_list_contents:
-        forall loc ts,
-          (<<NORMAL: sim_promise_content_strong (self loc ts) (extra loc ts) (extra_all loc) loc ts
-                                                (Memory.get loc ts prom_src)
-                                                (Memory.get loc ts prom_tgt)>>) \/
-          ((<<LIN: List.In (loc, ts) l>>) /\
-           (<<WEAK: sim_promise_content (self loc ts) (extra loc ts) loc ts
-                                        (Memory.get loc ts prom_src)
-                                        (Memory.get loc ts prom_tgt)>>));
-      sim_promise_list_wf:
-        forall loc from ts (EXTRA: extra loc ts from),
-          (<<FORGET: self loc from>>) /\
-          (<<LB: lb_time (times loc) from ts>>) /\
-          (<<TS: Time.lt from ts>>);
-      sim_promise_list_extra:
-        forall loc ts (SELF: self loc ts),
-        exists to,
-          (<<GET: Memory.get loc to prom_src = Some (ts, Message.reserve)>>) /\
-          (<<TS: Time.lt ts to>>);
-    }.
-
-  Lemma sim_promise_list_nil self extra extra_all prom_src prom_tgt
-        (SIM: sim_promise_list self extra extra_all prom_src prom_tgt [])
-    :
-      sim_promise_strong self extra extra_all prom_src prom_tgt.
-  Proof.
-    econs.
-    - ii. hexploit SIM.(sim_promise_list_contents); eauto. i. des; eauto. ss.
-    - apply SIM.
-    - apply SIM.
-  Qed.
-
-  Lemma sim_promise_weak_list_exists self extra extra_all prom_src prom_tgt
-        (SIM: sim_promise self extra prom_src prom_tgt)
-        (FIN: Memory.finite prom_src)
-    :
-      exists l,
-        (<<SIM: sim_promise_list self extra extra_all prom_src prom_tgt l>>).
-  Proof.
-    unfold Memory.finite in *. des.
-    hexploit (@list_filter_exists
-                (Loc.t * Time.t)
-                (fun locts =>
-                   let (loc, ts) := locts in
-                   ~ sim_promise_content_strong (self loc ts) (extra loc ts) (extra_all loc) loc ts
-                     (Memory.get loc ts prom_src)
-                     (Memory.get loc ts prom_tgt))
-                dom).
-    i. des. exists l'. econs; [|apply SIM|apply SIM].
-    ii. set (PROM:= SIM.(sim_promise_contents) loc ts).
-    destruct (classic (List.In (loc,ts) l')).
-    - right. splits; auto.
-    - left. red. inv PROM; try by (econs; eauto).
-      + apply NNPP. ii. exploit FIN; eauto. i.
-        hexploit (proj1 (@COMPLETE (loc, ts))); auto.
-        splits; auto. ii. rewrite H1 in *. rewrite H2 in *. auto.
-      + apply NNPP. ii. exploit FIN; eauto. i.
-        hexploit (proj1 (@COMPLETE (loc, ts))); auto.
-        splits; auto. ii. rewrite H1 in *. rewrite H2 in *. auto.
-  Qed.
-
-  Lemma reserve_future_memory_unch
-        prom0 mem0 prom1 mem1
-        (FUTURE: reserve_future_memory prom0 mem0 prom1 mem1)
-        loc to from msg
-        (GETMEM: Memory.get loc to mem0 = Some (from, msg))
-        (GETPROM: Memory.get loc to prom0 = None)
-    :
-      (<<GETMEM: Memory.get loc to mem1 = Some (from, msg)>>) /\
-      (<<GETPROM: Memory.get loc to prom1 = None>>).
-  Proof.
-    ginduction FUTURE; eauto. i. inv HD; clarify.
-    { eapply IHFUTURE; eauto.
-      - erewrite Memory.add_o; eauto. des_ifs.
-        ss. des; clarify.
-        eapply Memory.add_get0 in MEM. des. clarify.
-      - erewrite Memory.add_o; eauto. des_ifs.
-        ss. des; clarify.
-        eapply Memory.add_get0 in MEM. des. clarify. }
-    { apply split_succeed_wf in PROMISES. des. clarify. }
-    { apply lower_succeed_wf in PROMISES. des. clarify. inv MSG_LE. }
-    { eapply IHFUTURE; eauto.
-      - erewrite Memory.remove_o; eauto. des_ifs.
-        ss. des; clarify.
-        eapply Memory.remove_get0 in PROMISES. des. clarify.
-      - erewrite Memory.remove_o; eauto. des_ifs. }
-  Qed.
-
   Lemma sim_memory_get_larger F extra mem_src mem_tgt loc from_src ts msg_src
         (MEM: sim_memory F extra mem_src mem_tgt)
         (GETSRC: Memory.get loc ts mem_src = Some (from_src, msg_src))
@@ -855,22 +408,6 @@ Section SIM.
       apply MEM.(sim_memory_wf) in EXTRA. des; auto. }
   Qed.
 
-  Lemma memory_get_disjoint_strong mem loc from0 to0 from1 to1 msg0 msg1
-        (GET0: Memory.get loc to0 mem = Some (from0, msg0))
-        (GET1: Memory.get loc to1 mem = Some (from1, msg1))
-    :
-      (to0 = to1 /\ from0 = from1 /\ msg0 = msg1) \/
-      (<<TS: Time.le to0 from1>> /\ <<TS: Time.lt to0 to1>>) \/
-      (<<TS: Time.le to1 from0>> /\ <<TS: Time.lt to1 to0>>).
-  Proof.
-    destruct (Time.le_lt_dec to0 to1).
-    { destruct l.
-      { dup H. eapply memory_get_from_mon in H; eauto. }
-      { inv H. clarify. auto. }
-    }
-    { dup l. eapply memory_get_from_mon in l; eauto. }
-  Qed.
-
   Lemma memory_forget_extra_exclusive F extra mem_src mem_tgt loc from to ts
         (MEM: sim_memory F extra mem_src mem_tgt)
         (FORGET: F loc ts)
@@ -883,41 +420,11 @@ Section SIM.
     eapply NEXTRA; eauto.
   Qed.
 
-  Lemma promises_forget_extra_exclusive F extra mem_src mem_tgt loc from to ts
-        (PROMISES: sim_promise F extra mem_src mem_tgt)
-        (FORGET: F loc ts)
-        (EXTRA: extra loc to from)
-    :
-      ts <> to.
-  Proof.
-    ii. subst.
-    set (PROM:=PROMISES.(sim_promise_contents) loc to). inv PROM; ss.
-    eapply NEXTRA; eauto.
-  Qed.
-
-  Definition memory_times_wf (mem: Memory.t): Prop :=
-    forall loc to from msg
-           (GET: Memory.get loc to mem = Some (from, msg)),
-      (<<FROM: List.In from (times loc)>>) /\ (<<TO: List.In to (times loc)>>).
-
-  Definition memory_times_wf_strong (mem: Memory.t): Prop :=
-    forall loc to from msg
-           (GET: Memory.get loc to mem = Some (from, msg)),
-      (<<FROM: List.In from (times loc)>>) /\ (<<TO: List.In to (times loc)>>) /\
-      (<<CAP: List.In (Time.incr to) (times loc)>>).
-
-  Lemma memory_times_wf_strong_wf
-    :
-      memory_times_wf_strong <1= memory_times_wf.
-  Proof.
-    ii. eapply PR in GET. des. auto.
-  Qed.
-
   Lemma sim_memory_disjoint F extra mem_src mem_tgt
         loc from_tgt to_tgt msg_tgt
         from_src to_src msg_src x
         (MEM: sim_memory F extra mem_src mem_tgt)
-        (MEMWF: memory_times_wf mem_tgt)
+        (MEMWF: memory_times_wf times mem_tgt)
         (GETTGT: Memory.get loc to_tgt mem_tgt = Some (from_tgt, msg_tgt))
         (GETSRC: Memory.get loc to_src mem_src = Some (from_src, msg_src))
         (ITVTGT: Interval.mem (from_tgt, to_tgt) x)
@@ -1067,6 +574,92 @@ Section SIM.
     rewrite GETSRC in MEM0. inv MEM0. splits; auto.
   Qed.
 
+
+
+  (* sim promises *)
+
+  Inductive sim_promise_content
+            (F: Prop)
+            (extra: Time.t -> Prop)
+            (loc: Loc.t) (ts: Time.t)
+    :
+      option (Time.t * Message.t) -> option (Time.t * Message.t) -> Prop :=
+  | sim_promise_content_none
+      (NPROM: ~ F)
+      (NEXTRA: forall t, ~ extra t)
+      (NLOC: L loc)
+    :
+      sim_promise_content F extra loc ts None None
+  | sim_promise_content_normal
+      (NPROM: ~ F)
+      (NEXTRA: forall t, ~ extra t)
+      (NLOC: ~ L loc)
+      cnt
+    :
+      sim_promise_content F extra loc ts cnt cnt
+  | sim_promise_content_reserve
+      (NPROM: ~ F)
+      (NEXTRA: forall t, ~ extra t)
+      (LOC: L loc)
+      from_src from_tgt
+    :
+      sim_promise_content F extra loc ts
+                          (Some (from_src, Message.reserve))
+                          (Some (from_tgt, Message.reserve))
+  | sim_promise_content_forget
+      (PROM: F)
+      (NEXTRA: forall t, ~ extra t)
+      (LOC: L loc)
+      from_src from_tgt val released
+    :
+      sim_promise_content F extra loc ts
+                          (Some (from_src, Message.reserve))
+                          (Some (from_tgt, Message.concrete val released))
+  | sim_promise_content_extra
+      from
+      (NPROM: ~ F)
+      (LOC: L loc)
+      (EXTRA: extra from)
+    :
+      sim_promise_content F extra loc ts (Some (from, Message.reserve)) None
+  .
+  Hint Constructors sim_promise_content.
+
+  Record sim_promise
+         (self: Loc.t -> Time.t -> Prop)
+         (extra: Loc.t -> Time.t -> Time.t -> Prop)
+         (prom_src prom_tgt: Memory.t): Prop :=
+    {
+      sim_promise_contents:
+        forall loc ts,
+          sim_promise_content (self loc ts) (extra loc ts)
+                              loc ts
+                              (Memory.get loc ts prom_src)
+                              (Memory.get loc ts prom_tgt);
+      sim_promise_wf:
+        forall loc from ts (EXTRA: extra loc ts from),
+          (<<FORGET: self loc from>>) /\
+          (<<LB: lb_time (times loc) from ts>>) /\
+          (<<TS: Time.lt from ts>>);
+      sim_promise_extra:
+        forall loc ts (SELF: self loc ts),
+        exists to,
+          (<<GET: Memory.get loc to prom_src = Some (ts, Message.reserve)>>) /\
+          (<<TS: Time.lt ts to>>);
+    }.
+
+  Lemma promises_forget_extra_exclusive F extra mem_src mem_tgt loc from to ts
+        (PROMISES: sim_promise F extra mem_src mem_tgt)
+        (FORGET: F loc ts)
+        (EXTRA: extra loc to from)
+    :
+      ts <> to.
+  Proof.
+    ii. subst.
+    set (PROM:=PROMISES.(sim_promise_contents) loc to). inv PROM; ss.
+    eapply NEXTRA; eauto.
+  Qed.
+
   Lemma sim_promise_src_none F extra prom_src prom_tgt
         (PROMISE: sim_promise F extra prom_src prom_tgt)
         loc to
@@ -1082,6 +675,174 @@ Section SIM.
     - splits; auto.
   Qed.
 
+
+
+  (* sim promises strong *)
+
+  Inductive sim_promise_content_strong
+            (F: Prop)
+            (extra: Time.t -> Prop)
+            (extra_all: Time.t -> Time.t -> Prop)
+            (loc: Loc.t) (ts: Time.t)
+    :
+      option (Time.t * Message.t) -> option (Time.t * Message.t) -> Prop :=
+  | sim_promise_content_strong_none
+      (NPROM: ~ F)
+      (NEXTRA: forall t, ~ extra t)
+      (NLOC: L loc)
+    :
+      sim_promise_content_strong F extra extra_all loc ts None None
+  | sim_promise_content_strong_normal
+      (NPROM: ~ F)
+      (NEXTRA: forall t, ~ extra t)
+      (NLOC: ~ L loc)
+      cnt
+    :
+      sim_promise_content_strong F extra extra_all loc ts cnt cnt
+  | sim_promise_content_strong_reserve
+      (NPROM: ~ F)
+      (NEXTRA: forall t, ~ extra t)
+      (LOC: L loc)
+      from_src from_tgt
+      (EXTRA: from_tgt = from_src \/ extra_all from_src from_tgt)
+    :
+      sim_promise_content_strong F extra extra_all loc ts
+                          (Some (from_src, Message.reserve))
+                          (Some (from_tgt, Message.reserve))
+  | sim_promise_content_strong_forget
+      (PROM: F)
+      (NEXTRA: forall t, ~ extra t)
+      (LOC: L loc)
+      from_src from_tgt val released
+      (EXTRA: from_tgt = from_src \/ extra_all from_src from_tgt)
+    :
+      sim_promise_content_strong F extra extra_all loc ts
+                          (Some (from_src, Message.reserve))
+                          (Some (from_tgt, Message.concrete val released))
+  | sim_promise_content_strong_extra
+      from
+      (NPROM: ~ F)
+      (LOC: L loc)
+      (EXTRA: extra from)
+    :
+      sim_promise_content_strong F extra extra_all loc ts (Some (from, Message.reserve)) None
+  .
+  Hint Constructors sim_promise_content_strong.
+
+  Lemma sim_promise_content_strong_sim_promise_content
+        loc ts F extra get0 get1 extra_all
+        (SIM: sim_promise_content_strong F extra extra_all loc ts  get0 get1)
+    :
+      sim_promise_content F extra loc ts get0 get1.
+  Proof.
+    inv SIM; econs; eauto.
+  Qed.
+
+  Record sim_promise_strong
+         (self: Loc.t -> Time.t -> Prop)
+         (extra: Loc.t -> Time.t -> Time.t -> Prop)
+         (extra_all: Loc.t -> Time.t -> Time.t -> Prop)
+         (prom_src prom_tgt: Memory.t): Prop :=
+    {
+      sim_promise_strong_contents:
+        forall loc ts,
+          sim_promise_content_strong (self loc ts) (extra loc ts) (extra_all loc)
+                                     loc ts
+                                     (Memory.get loc ts prom_src)
+                                     (Memory.get loc ts prom_tgt);
+      sim_promise_strong_wf:
+        forall loc from ts (EXTRA: extra loc ts from),
+          (<<FORGET: self loc from>>) /\
+          (<<LB: lb_time (times loc) from ts>>) /\
+          (<<TS: Time.lt from ts>>);
+      sim_promise_strong_extra:
+        forall loc ts (SELF: self loc ts),
+        exists to,
+          (<<GET: Memory.get loc to prom_src = Some (ts, Message.reserve)>>) /\
+          (<<TS: Time.lt ts to>>);
+    }.
+
+  Lemma sim_promise_strong_sim_promise
+        self extra extra_all prom_src prom_tgt
+        (SIM: sim_promise_strong self extra extra_all prom_src prom_tgt)
+    :
+      sim_promise self extra prom_src prom_tgt.
+  Proof.
+    econs.
+    - ii. eapply sim_promise_content_strong_sim_promise_content; eauto.
+      eapply SIM; eauto.
+    - apply SIM.
+    - apply SIM.
+  Qed.
+
+  Record sim_promise_list
+         (self: Loc.t -> Time.t -> Prop)
+         (extra: Loc.t -> Time.t -> Time.t -> Prop)
+         (extra_all: Loc.t -> Time.t -> Time.t -> Prop)
+         (prom_src prom_tgt: Memory.t)
+         (l: list (Loc.t * Time.t)): Prop :=
+    {
+      sim_promise_list_contents:
+        forall loc ts,
+          (<<NORMAL: sim_promise_content_strong (self loc ts) (extra loc ts) (extra_all loc) loc ts
+                                                (Memory.get loc ts prom_src)
+                                                (Memory.get loc ts prom_tgt)>>) \/
+          ((<<LIN: List.In (loc, ts) l>>) /\
+           (<<WEAK: sim_promise_content (self loc ts) (extra loc ts) loc ts
+                                        (Memory.get loc ts prom_src)
+                                        (Memory.get loc ts prom_tgt)>>));
+      sim_promise_list_wf:
+        forall loc from ts (EXTRA: extra loc ts from),
+          (<<FORGET: self loc from>>) /\
+          (<<LB: lb_time (times loc) from ts>>) /\
+          (<<TS: Time.lt from ts>>);
+      sim_promise_list_extra:
+        forall loc ts (SELF: self loc ts),
+        exists to,
+          (<<GET: Memory.get loc to prom_src = Some (ts, Message.reserve)>>) /\
+          (<<TS: Time.lt ts to>>);
+    }.
+
+  Lemma sim_promise_list_nil self extra extra_all prom_src prom_tgt
+        (SIM: sim_promise_list self extra extra_all prom_src prom_tgt [])
+    :
+      sim_promise_strong self extra extra_all prom_src prom_tgt.
+  Proof.
+    econs.
+    - ii. hexploit SIM.(sim_promise_list_contents); eauto. i. des; eauto. ss.
+    - apply SIM.
+    - apply SIM.
+  Qed.
+
+  Lemma sim_promise_weak_list_exists self extra extra_all prom_src prom_tgt
+        (SIM: sim_promise self extra prom_src prom_tgt)
+        (FIN: Memory.finite prom_src)
+    :
+      exists l,
+        (<<SIM: sim_promise_list self extra extra_all prom_src prom_tgt l>>).
+  Proof.
+    unfold Memory.finite in *. des.
+    hexploit (@list_filter_exists
+                (Loc.t * Time.t)
+                (fun locts =>
+                   let (loc, ts) := locts in
+                   ~ sim_promise_content_strong (self loc ts) (extra loc ts) (extra_all loc) loc ts
+                     (Memory.get loc ts prom_src)
+                     (Memory.get loc ts prom_tgt))
+                dom).
+    i. des. exists l'. econs; [|apply SIM|apply SIM].
+    ii. set (PROM:= SIM.(sim_promise_contents) loc ts).
+    destruct (classic (List.In (loc,ts) l')).
+    - right. splits; auto.
+    - left. red. inv PROM; try by (econs; eauto).
+      + apply NNPP. ii. exploit FIN; eauto. i.
+        hexploit (proj1 (@COMPLETE (loc, ts))); auto.
+        splits; auto. ii. rewrite H1 in *. rewrite H2 in *. auto.
+      + apply NNPP. ii. exploit FIN; eauto. i.
+        hexploit (proj1 (@COMPLETE (loc, ts))); auto.
+        splits; auto. ii. rewrite H1 in *. rewrite H2 in *. auto.
+  Qed.
+
   Lemma sim_promise_weak_stengthen others self extra_others extra_self
         prom_src prom_tgt mem_src mem_tgt
         (MEM: sim_memory (others \\2// self) (extra_others \\3// extra_self) mem_src mem_tgt)
@@ -1090,8 +851,7 @@ Section SIM.
         (FIN: Memory.finite prom_src)
         (BOTNONESRC: Memory.bot_none prom_src)
         (PROM: sim_promise self extra_self prom_src prom_tgt)
-        (* (SELF: self <2= promised prom_src) *)
-        (MEMWF: memory_times_wf mem_tgt)
+        (MEMWF: memory_times_wf times mem_tgt)
     :
       exists prom_src' mem_src',
         (<<FUTURE: reserve_future_memory prom_src mem_src prom_src' mem_src'>>) /\
@@ -1396,7 +1156,397 @@ Section SIM.
   Qed.
 
 
-  Lemma sim_promise_step_forget others self extra_others extra_self
+
+  (* sim local *)
+
+  Inductive sim_local
+            (self: Loc.t -> Time.t -> Prop)
+            (extra: Loc.t -> Time.t -> Time.t -> Prop)
+    :
+      forall (lc_src lc_tgt: Local.t), Prop :=
+  | sim_local_intro
+      tvw prom_src prom_tgt
+      (PROMS: sim_promise self extra prom_src prom_tgt)
+    :
+      sim_local self extra (Local.mk tvw prom_src) (Local.mk tvw prom_tgt)
+  .
+  Hint Constructors sim_local.
+
+  Inductive sim_statelocal
+            (self: Loc.t -> Time.t -> Prop)
+            (extra: Loc.t -> Time.t -> Time.t -> Prop)
+    :
+      sigT (@Language.state ProgramEvent.t) * Local.t -> sigT (@Language.state ProgramEvent.t) * Local.t -> Prop :=
+  | forget_statelocal_intro
+      st lc_src lc_tgt
+      (LOCAL: sim_local self extra lc_src lc_tgt)
+    :
+      sim_statelocal self extra (st, lc_src) (st, lc_tgt)
+  .
+
+
+
+  Lemma sim_read_step extra self others lc_src lc_tgt mem_src mem_tgt loc to val released ord
+        lc_tgt'
+        (STEPTGT: Local.read_step lc_tgt mem_tgt loc to val released ord lc_tgt')
+        (NOREAD: ~ others loc to)
+        (MEM: sim_memory (others \\2// self) extra mem_src mem_tgt)
+        (LOCAL: sim_local self extra lc_src lc_tgt)
+        (CLOSED: Memory.closed mem_src)
+        (CONSISTENT: Local.promise_consistent lc_tgt')
+    :
+      exists lc_src',
+        (<<STEPSRC: Local.read_step lc_src mem_src loc to val released ord lc_src'>>) /\
+        (<<SIM: sim_local self extra lc_src' lc_tgt'>>) /\
+        (<<GETSRC: exists from, Memory.get loc to mem_src = Some (from, Message.concrete val released)>>) /\
+        (<<GETTGT: exists from, Memory.get loc to mem_tgt = Some (from, Message.concrete val released)>>) /\
+        (<<RELEASEDMCLOSED: Memory.closed_opt_view released mem_src>>) /\
+        (<<RELEASEDMWF: View.opt_wf released>>) /\
+        (<<NOREAD: ~ (others \\2// self) loc to>>)
+  .
+  Proof.
+    inv LOCAL. inv STEPTGT.
+    set (MEM0:= MEM.(sim_memory_contents) loc to). rewrite GET in *. inv MEM0; ss.
+    { inv CLOSED. hexploit CLOSED0.
+      { symmetry.  eapply H0. } i. des. inv MSG_CLOSED. inv MSG_WF.
+      esplits; eauto. }
+    { exfalso. destruct PROM; auto.
+      set (PROM:= PROMS.(sim_promise_contents) loc to). inv PROM; ss.
+      symmetry in H3. eapply CONSISTENT in H3. ss.
+      eapply Time.lt_strorder. eapply TimeFacts.lt_le_lt; [apply H3|].
+      unfold TimeMap.join, View.singleton_ur_if, View.singleton_ur, View.singleton_rw, TimeMap.singleton.
+      etrans; [|eapply Time.join_l]. etrans; [|eapply Time.join_r].
+      des_ifs; ss; setoid_rewrite LocFun.add_spec_eq; refl.
+    }
+  Qed.
+
+  Lemma sim_fence_step self extra lc_src lc_tgt sc ordr ordw
+        sc' lc_tgt'
+        (STEPTGT: Local.fence_step lc_tgt sc ordr ordw lc_tgt' sc')
+        (LOCAL: sim_local self extra lc_src lc_tgt)
+    :
+      exists lc_src',
+        (<<STEPSRC: Local.fence_step lc_src sc ordr ordw lc_src' sc'>>) /\
+        (<<SIM: sim_local self extra lc_src' lc_tgt'>>)
+  .
+  Proof.
+    inv LOCAL. inv STEPTGT. esplits.
+    - econs; ss; eauto. ii.
+      set (PROM:= PROMS.(sim_promise_contents) loc t).
+      rewrite GET in *. inv PROM; ss.
+      exploit RELEASE; eauto.
+    - econs; ss; eauto.
+  Qed.
+
+  Lemma sim_promise_consistent self extra lc_src lc_tgt
+        (CONSISTENT: Local.promise_consistent lc_tgt)
+        (SIM: sim_local self extra lc_src lc_tgt)
+    :
+      Local.promise_consistent lc_src.
+  Proof.
+    inv SIM. ii. ss.
+    set (PROM:= PROMS.(sim_promise_contents) loc ts).
+    rewrite PROMISE in *. inv PROM. eauto.
+  Qed.
+
+  Lemma sim_failure_step self extra lc_src lc_tgt
+        (STEPTGT: Local.failure_step lc_tgt)
+        (SIM: sim_local self extra lc_src lc_tgt)
+    :
+      Local.failure_step lc_src.
+  Proof.
+    inv STEPTGT. econs.
+    eapply sim_promise_consistent; eauto.
+  Qed.
+
+  Lemma sim_promise_normal others self extra_others extra_self
+        mem_src mem_tgt prom_src prom_tgt
+        loc from to msg prom_tgt' mem_tgt' kind
+        (NLOC: ~ L loc)
+        (STEPTGT: Memory.promise prom_tgt mem_tgt loc from to msg prom_tgt' mem_tgt' kind)
+        (MEM: sim_memory (others \\2// self) (extra_others \\3// extra_self) mem_src mem_tgt)
+        (MEMSRC: Memory.closed mem_src)
+        (MEMTGT: Memory.closed mem_tgt)
+        (WFSRC: Memory.le prom_src mem_src)
+        (WFTGT: Memory.le prom_tgt mem_tgt)
+        (PROMISE: sim_promise self extra_self prom_src prom_tgt)
+        (SEMI: semi_closed_message msg mem_src loc to)
+    :
+      exists prom_src' mem_src',
+        (<<STEPSRC: Memory.promise prom_src mem_src loc from to msg prom_src' mem_src' kind>>) /\
+        (<<MEM: sim_memory (others \\2// self) (extra_others \\3// extra_self) mem_src' mem_tgt'>>) /\
+        (<<PROMISE: sim_promise self extra_self prom_src' prom_tgt'>>) /\
+        (<<CLOSED: Memory.closed_message msg mem_src'>>)
+  .
+  Proof.
+    generalize (sim_memory_others_self_wf MEM). intros PROMSWF.
+    generalize (sim_memory_extra_others_self_wf MEM). intros EXTRAWF.
+    inv STEPTGT.
+
+    (* add case *)
+    - exploit add_succeed_wf; try apply MEM0. i. des.
+      hexploit (@Memory.add_exists mem_src loc from to msg); ss.
+      { i. set (MEM1:= MEM.(sim_memory_contents) loc to2).
+        rewrite GET2 in *. inv MEM1; cycle 1.
+        { exfalso. apply NLOC. des; eauto. }
+        { exfalso. apply NLOC. des; eauto. }
+        ii. eapply DISJOINT; eauto.
+        inv RHS. econs; ss. eapply TimeFacts.le_lt_lt; eauto. }
+      intros [mem_src' ADDMEMSRC].
+      exploit Memory.add_exists_le; try apply ADDMEMSRC; eauto.
+      intros [prom_src' ADDPROMSRC].
+
+      assert (PROMISESRC: Memory.promise prom_src mem_src loc from to msg prom_src' mem_src' Memory.op_kind_add).
+      { econs; eauto. i. subst.
+        set (MEM1:= MEM.(sim_memory_contents) loc to'). rewrite GET in MEM1. inv MEM1; ss.
+        eapply ATTACH; eauto. erewrite NLOC0; eauto. }
+
+      assert (CLOSEDMSG: Memory.closed_message msg mem_src').
+      { destruct msg; auto.
+        eapply semi_closed_message_add; eauto. }
+
+      exists prom_src', mem_src'. splits; auto.
+      + econs.
+        { ii. set (MEM1:= MEM.(sim_memory_contents) loc0 ts).
+          erewrite (@Memory.add_o mem_src'); eauto.
+          erewrite (@Memory.add_o mem_tgt'); eauto.
+          des_ifs; try by (ss; des; clarify).
+          * econs; eauto.
+            { ii. ss. des; clarify; eauto. }
+            { ii. ss. des; clarify; eauto. }
+            { refl. }
+            { i. ss. }
+        }
+        { eapply MEM.(sim_memory_wf); eauto. }
+      + econs.
+        { ii. set (PROM:= PROMISE.(sim_promise_contents) loc0 ts).
+          erewrite (@Memory.add_o prom_src'); eauto.
+          erewrite (@Memory.add_o prom_tgt'); eauto. des_ifs.
+          ss. des; clarify. econs; eauto.
+          { ii. eapply NLOC. eapply PROMSWF; ss. right. eauto. }
+          { ii. eapply NLOC. eapply EXTRAWF; ss. right. eauto. }
+        }
+        { apply PROMISE. }
+        { i. hexploit PROMISE.(sim_promise_extra); eauto. i. des.
+          esplits; eauto. erewrite (@Memory.add_o prom_src'); eauto.
+          des_ifs. ss. des; clarify.
+          exfalso. eapply NLOC. eapply PROMSWF; eauto. right. eauto. }
+
+    (* split case *)
+    - exploit split_succeed_wf; try apply PROMISES. i. des. clarify.
+      set (PROMISE0:= PROMISE.(sim_promise_contents) loc ts3). rewrite GET2 in *.
+      inv PROMISE0; ss.
+      hexploit (@Memory.split_exists prom_src loc from to ts3 (Message.concrete val' released')); ss.
+      { eauto. }
+      intros [prom_src' SPLITPROMSRC].
+      exploit Memory.split_exists_le; try apply SPLITPROMSRC; eauto.
+      intros [mem_src' SPLITMEMSRC].
+
+      assert (PROMISESRC: Memory.promise prom_src mem_src loc from to (Message.concrete val' released') prom_src' mem_src' (Memory.op_kind_split ts3 msg3)).
+      { econs; eauto. }
+
+      assert (CLOSEDMSG: Memory.closed_message (Message.concrete val' released') mem_src').
+      { eapply semi_closed_message_split; eauto. }
+
+      exists prom_src', mem_src'. splits; auto.
+      + econs.
+        { ii. set (MEM1:=MEM.(sim_memory_contents) loc0 ts).
+          erewrite (@Memory.split_o mem_src'); eauto.
+          erewrite (@Memory.split_o mem_tgt'); eauto.
+          des_ifs; try by (ss; des; clarify).
+          { ss. des; clarify. econs; eauto.
+            * refl.
+            * i. ss. }
+          { guardH o. ss. des; clarify. econs; eauto.
+            * refl.
+            * i. ss. }
+        }
+        { apply MEM.(sim_memory_wf); eauto. }
+      + econs.
+        { ii. set (PROM:= PROMISE.(sim_promise_contents) loc0 ts).
+          erewrite (@Memory.split_o prom_src'); eauto.
+          erewrite (@Memory.split_o prom_tgt'); eauto. des_ifs.
+          * ss. des; clarify. econs; eauto.
+            { ii. eapply NLOC. eapply PROMSWF. right. eauto. }
+            { ii. eapply NLOC. eapply EXTRAWF. right. eauto. }
+          * guardH o. ss. des; clarify. econs; eauto. }
+        { apply PROMISE. }
+        { i. hexploit PROMISE.(sim_promise_extra); eauto. i. des.
+          esplits; eauto. erewrite (@Memory.split_o prom_src'); eauto. des_ifs.
+          - ss. des; clarify. exfalso. eapply NLOC. eapply PROMSWF; eauto. right. eauto.
+          - ss. des; clarify. exfalso. eapply NLOC. eapply PROMSWF; eauto. right. eauto. }
+
+    (* lower case *)
+    - exploit lower_succeed_wf; try apply PROMISES. i. des. clarify.
+      set (PROMISE0:= PROMISE.(sim_promise_contents) loc to). rewrite GET in *. inv PROMISE0; ss.
+
+      hexploit (@Memory.lower_exists prom_src loc from to (Message.concrete val released) msg); ss.
+
+      intros [prom_src' LOWERPROMSRC].
+      exploit Memory.lower_exists_le; try apply LOWERPROMSRC; eauto.
+      intros [mem_src' LOWERMEMSRC].
+
+      assert (PROMISESRC: Memory.promise prom_src mem_src loc from to msg prom_src' mem_src' (Memory.op_kind_lower (Message.concrete val released))).
+      { econs; eauto. }
+
+      assert (CLOSEDMSG: Memory.closed_message msg mem_src').
+      { destruct msg; auto.
+        eapply semi_closed_message_lower; eauto. }
+
+      exists prom_src', mem_src'. splits; auto.
+      + econs.
+        { ii. set (MEM1:=MEM.(sim_memory_contents) loc0 ts).
+          erewrite (@Memory.lower_o mem_src'); eauto.
+          erewrite (@Memory.lower_o mem_tgt'); eauto. des_ifs.
+          ss. des; clarify. econs; eauto.
+          * refl.
+          * i. ss. }
+        { apply MEM.(sim_memory_wf); eauto. }
+      + econs.
+        { ii. set (PROM:= PROMISE.(sim_promise_contents) loc0 ts).
+          erewrite (@Memory.lower_o prom_src'); eauto.
+          erewrite (@Memory.lower_o prom_tgt'); eauto. des_ifs.
+          ss. des; clarify. econs; eauto. }
+        { apply PROMISE. }
+        { i. hexploit PROMISE.(sim_promise_extra); eauto. i. des.
+          esplits; eauto. erewrite (@Memory.lower_o prom_src'); eauto. des_ifs.
+          ss. des; clarify. }
+
+    (* cancel case *)
+    - exploit Memory.remove_get0; try apply PROMISES. i. des.
+      set (PROMISE0 := PROMISE.(sim_promise_contents) loc to). rewrite GET in *.
+      inv PROMISE0; ss.
+
+      hexploit (@Memory.remove_exists prom_src loc from to Message.reserve); ss.
+      intros [prom_src' REMOVEPROMSRC].
+      exploit Memory.remove_exists_le; try apply REMOVEPROMSRC; eauto.
+      intros [mem_src' REMOVEMEMSRC].
+
+      assert (PROMISESRC: Memory.promise prom_src mem_src loc from to Message.reserve prom_src' mem_src' Memory.op_kind_cancel).
+      { econs; eauto. }
+
+      exists prom_src', mem_src'.
+      splits; auto.
+      + econs.
+        { ii. set (MEM1:=MEM.(sim_memory_contents) loc0 ts).
+          erewrite (@Memory.remove_o mem_src'); eauto.
+          erewrite (@Memory.remove_o mem_tgt'); eauto.
+          des_ifs; try by (des; ss; clarify).
+          * ss. des; clarify. econs; eauto. }
+        { apply MEM. }
+      + econs.
+        { ii. set (PROM:= PROMISE.(sim_promise_contents) loc0 ts).
+          erewrite (@Memory.remove_o prom_src'); eauto.
+          erewrite (@Memory.remove_o prom_tgt'); eauto. des_ifs.
+          ss. des; clarify. econs 2; eauto. }
+        { apply PROMISE. }
+        { i. hexploit PROMISE.(sim_promise_extra); eauto. i. des.
+          esplits; eauto. erewrite (@Memory.remove_o prom_src'); eauto. des_ifs.
+          ss. des; clarify. exfalso. eapply NLOC. eapply PROMSWF; eauto. right. eauto. }
+  Qed.
+
+
+  Lemma sim_write_step_normal
+        others self extra_others extra_self lc_src lc_tgt sc mem_src mem_tgt
+        lc_tgt' sc' mem_tgt' loc from to val ord releasedm released kind
+        (NLOC: ~ L loc)
+        (STEPTGT: Local.write_step lc_tgt sc mem_tgt loc from to val releasedm released ord lc_tgt' sc' mem_tgt' kind)
+        (MEM: sim_memory (others \\2// self) (extra_others \\3// extra_self) mem_src mem_tgt)
+        (SCSRC: Memory.closed_timemap sc mem_src)
+        (SCTGT: Memory.closed_timemap sc mem_tgt)
+        (MEMSRC: Memory.closed mem_src)
+        (MEMTGT: Memory.closed mem_tgt)
+        (LOCALSRC: Local.wf lc_src mem_src)
+        (LOCALTGT: Local.wf lc_tgt mem_tgt)
+        (SIM: sim_local self extra_self lc_src lc_tgt)
+
+        (RELEASEDMCLOSED: Memory.closed_opt_view releasedm mem_src)
+        (RELEASEDMWF: View.opt_wf releasedm)
+    :
+      exists lc_src' mem_src',
+        (<<STEPSRC: Local.write_step lc_src sc mem_src loc from to val releasedm released ord lc_src' sc' mem_src' kind>>) /\
+        (<<MEM: sim_memory (others \\2// self) (extra_others \\3// extra_self) mem_src' mem_tgt'>>) /\
+        (<<SIM: sim_local self extra_self lc_src' lc_tgt'>>)
+  .
+  Proof.
+    inv STEPTGT. inv WRITE. inv SIM. inv LOCALSRC. inv LOCALTGT.
+
+    hexploit sim_promise_normal; eauto.
+    { ss. econs. unfold TView.write_released. des_ifs; econs.
+      eapply semi_closed_view_join.
+      - inv MEMSRC. eapply unwrap_closed_opt_view; auto.
+        eapply closed_opt_view_semi_closed. auto.
+      - ss. setoid_rewrite LocFun.add_spec_eq. des_ifs.
+        + eapply semi_closed_view_join.
+          * eapply closed_view_semi_closed. inv TVIEW_CLOSED. auto.
+          * inv MEMSRC. eapply semi_closed_view_singleton. auto.
+        + eapply semi_closed_view_join.
+          * eapply closed_view_semi_closed. inv TVIEW_CLOSED. auto.
+          * inv MEMSRC. eapply semi_closed_view_singleton. auto.
+    }
+    i. des. ss.
+
+    hexploit (@Memory.remove_exists
+                prom_src' loc from to
+                (Message.concrete val (TView.write_released tvw sc loc to releasedm ord))).
+    { set (PROM:= PROMISE0.(sim_promise_contents) loc to).
+      eapply Memory.remove_get0 in REMOVE. des.
+      rewrite GET in *. inv PROM; ss. }
+    intros [prom_src'' REMOVESRC].
+
+    assert (NSELF: forall ts, ~ self loc ts).
+    { ii. set (PROM:= PROMISE0.(sim_promise_contents) loc to). inv PROM; ss.
+      eapply NLOC. eapply sim_memory_others_self_wf; eauto. ss. right. eauto. }
+
+    esplits; eauto.
+
+    - econs; ss.
+      + econs; eauto.
+      + ii. set (PROM:=PROMS.(sim_promise_contents) loc t).
+        rewrite GET in *. inv PROM; ss.
+        exploit RELEASE; eauto.
+
+    - econs; auto. econs.
+      { ii. set (PROM:=PROMISE0.(sim_promise_contents) loc0 ts).
+        erewrite (@Memory.remove_o prom_src''); eauto.
+        erewrite (@Memory.remove_o promises2); eauto. des_ifs.
+        ss. des; subst. econs 2; eauto.
+        ii. exploit sim_memory_extra_others_self_wf.
+        { eapply MEM0. }
+        { right. eauto. }
+        { ii. ss. }
+      }
+      { apply PROMISE0. }
+      { i. set (PROM:=PROMISE0.(sim_promise_extra) loc0 ts SELF). des.
+        esplits; eauto. erewrite (@Memory.remove_o prom_src''); eauto.
+        des_ifs. ss. des; clarify. exfalso. eapply NSELF; eauto. }
+  Qed.
+
+  Lemma sim_promise_step_normal others self extra_others extra_self
+        mem_src mem_tgt mem_tgt' lc_src lc_tgt lc_tgt' loc from to msg kind
+        (NLOC: ~ L loc)
+        (STEPTGT: Local.promise_step lc_tgt mem_tgt loc from to msg lc_tgt' mem_tgt' kind)
+        (MEM: sim_memory (others \\2// self) (extra_others \\3// extra_self) mem_src mem_tgt)
+        (LOCAL: sim_local self extra_self lc_src lc_tgt)
+        (MEMSRC: Memory.closed mem_src)
+        (MEMTGT: Memory.closed mem_tgt)
+        (LCSRC: Local.wf lc_src mem_src)
+        (LCTGT: Local.wf lc_tgt mem_tgt)
+        (SEMI: semi_closed_message msg mem_src loc to)
+    :
+      exists lc_src' mem_src',
+        (<<STEPSRC: Local.promise_step lc_src mem_src loc from to msg lc_src' mem_src' kind>>) /\
+        (<<MEM: sim_memory (others \\2// self) (extra_others \\3// extra_self) mem_src' mem_tgt'>>) /\
+        (<<LOCAL: sim_local self extra_self lc_src' lc_tgt'>>)
+  .
+  Proof.
+    inv LOCAL. inv LCSRC. inv LCTGT. inv STEPTGT. ss.
+    hexploit sim_promise_normal; eauto. i. des.
+    exists (Local.mk tvw prom_src'), mem_src'. splits; eauto.
+  Qed.
+
+
+  Lemma sim_promise_forget others self extra_others extra_self
         mem_src mem_tgt prom_src prom_tgt
         loc from to msg_tgt prom_tgt' mem_tgt' kind_tgt
         (LOC: L loc)
@@ -1407,9 +1557,8 @@ Section SIM.
         (MLESRC: Memory.le prom_src mem_src)
         (MLETGT: Memory.le prom_tgt mem_tgt)
         (PROMISE: sim_promise self extra_self prom_src prom_tgt)
-        (PROMATTACH: promises_not_attached self (promised prom_src) mem_src)
 
-        (MEMWF: memory_times_wf mem_tgt')
+        (MEMWF: memory_times_wf times mem_tgt')
         (EXCLUSIVE: forall loc' ts' (OTHER: others loc' ts'),
             Memory.get loc' ts' prom_src = None)
         (EXCLUSIVEEXTRA: forall loc' ts' from' (EXTRA: extra_others loc' ts' from'),
@@ -2037,7 +2186,7 @@ Section SIM.
   Qed.
 
 
-  Lemma sim_promise_fulfill from_src' others self extra_others extra_self
+  Lemma sim_fulfill_forget from_src' others self extra_others extra_self
         prom_src prom_tgt mem_src mem_tgt prom_tgt'
         loc from_tgt to val released
         (LOC: L loc)
@@ -2059,7 +2208,7 @@ Section SIM.
                           (GET: Memory.get loc to mem_src = Some (from_src, msg))
                           ts (ITV: Interval.mem (from_src', from_src) ts),
             Memory.get loc ts mem_src = None)
-        (MEMWF: memory_times_wf mem_tgt)
+        (MEMWF: memory_times_wf times mem_tgt)
         (EXCLUSIVE: forall loc' ts' (OTHER: others loc' ts'),
             exists from msg, <<UNCH: unchangable mem_src prom_src loc' ts' from msg>>)
         (EXCLUSIVEEXTRA: forall loc' ts' from' (OTHER: extra_others loc' ts' from'),
@@ -2120,7 +2269,6 @@ Section SIM.
     { econs; eauto. }
 
     dup GETMEMTGT. eapply CLOSED in GETMEMTGT0. des.
-
 
     hexploit (@Memory.add_exists mem_src0 loc from_src' to (Message.concrete val released)); eauto.
     { ii. inv LHS. inv RHS. ss.
@@ -2361,7 +2509,8 @@ Section SIM.
     }
   Qed.
 
-  Lemma sim_promise_fulfill_write others self extra_others extra_self
+
+  Lemma sim_fulfill_forget_write others self extra_others extra_self
         prom_src prom_tgt mem_src mem_tgt prom_tgt'
         loc from_tgt to val released
         (LOC: L loc)
@@ -2375,7 +2524,7 @@ Section SIM.
         (REMOVE: Memory.remove prom_tgt loc from_tgt to (Message.concrete val released) prom_tgt')
         (CLOSED: Memory.closed mem_tgt)
 
-        (MEMWF: memory_times_wf mem_tgt)
+        (MEMWF: memory_times_wf times mem_tgt)
         (EXCLUSIVE: forall loc' ts' (OTHER: others loc' ts'),
             exists from msg, <<UNCH: unchangable mem_src prom_src loc' ts' from msg>>)
         (EXCLUSIVEEXTRA: forall loc' ts' from' (OTHER: extra_others loc' ts' from'),
@@ -2407,13 +2556,12 @@ Section SIM.
     rewrite GETMEMSRC in *. rewrite GETMEMTGT in *.
     inv MEM0; try by (exfalso; apply NPROM; right; auto).
 
-    exists from_src. eapply sim_promise_fulfill; eauto.
+    exists from_src. eapply sim_fulfill_forget; eauto.
     { i. clarify. refl. }
     { i. clarify. inv ITV. ss. timetac. }
   Qed.
 
-
-  Lemma sim_promise_fulfill_update others self extra_others extra_self
+  Lemma sim_fulfill_forget_update others self extra_others extra_self
         prom_src prom_tgt mem_src mem_tgt prom_tgt'
         loc from_tgt to val released
         (LOC: L loc)
@@ -2428,7 +2576,7 @@ Section SIM.
         (CLOSED: Memory.closed mem_tgt)
         (NOREAD: ~ (others \\2// self) loc from_tgt)
 
-        (MEMWF: memory_times_wf mem_tgt)
+        (MEMWF: memory_times_wf times mem_tgt)
         (EXCLUSIVE: forall loc' ts' (OTHER: others loc' ts'),
             exists from msg, <<UNCH: unchangable mem_src prom_src loc' ts' from msg>>)
         (EXCLUSIVEEXTRA: forall loc' ts' from' (OTHER: extra_others loc' ts' from'),
@@ -2460,7 +2608,7 @@ Section SIM.
     rewrite GETMEMSRC in *. rewrite GETMEMTGT in *.
     inv MEM0; try by (exfalso; apply NPROM; right; auto).
 
-    eapply sim_promise_fulfill; eauto.
+    eapply sim_fulfill_forget; eauto.
     { refl. }
     { i. clarify. }
     { i. clarify.
@@ -2515,6 +2663,82 @@ Section SIM.
   Qed.
 
 
+  Lemma sim_promise_step_forget others self extra_others extra_self
+        mem_src mem_tgt mem_tgt' lc_src lc_tgt lc_tgt' loc from to msg kind
+        (LOC: L loc)
+        (STEPTGT: Local.promise_step lc_tgt mem_tgt loc from to msg lc_tgt' mem_tgt' kind)
+        (MEM: sim_memory (others \\2// self) (extra_others \\3// extra_self) mem_src mem_tgt)
+        (LOCAL: sim_local self extra_self lc_src lc_tgt)
+        (MEMSRC: Memory.closed mem_src)
+        (MEMTGT: Memory.closed mem_tgt)
+        (LCSRC: Local.wf lc_src mem_src)
+        (LCTGT: Local.wf lc_tgt mem_tgt)
+
+        (CLOSED: Memory.closed mem_tgt)
+
+        (MEMWF: memory_times_wf times mem_tgt')
+        (CONSISTENT: Local.promise_consistent lc_tgt)
+        (EXCLUSIVE: forall loc' ts' (OTHER: others loc' ts'),
+            exists from msg, <<UNCH: unchangable mem_src lc_src.(Local.promises) loc' ts' from msg>>)
+        (EXCLUSIVEEXTRA: forall loc' ts' from' (OTHER: extra_others loc' ts' from'),
+            (<<UNCH: unchangable mem_src lc_src.(Local.promises) loc' ts' from' Message.reserve>>))
+    :
+      exists self' extra_self' prom_src' mem_src',
+        (<<FUTURE: reserve_future_memory lc_src.(Local.promises) mem_src prom_src' mem_src'>>) /\
+        (<<MEM: sim_memory (others \\2// self') (extra_others \\3// extra_self') mem_src' mem_tgt'>>) /\
+        (<<SIM: sim_local self' extra_self' (Local.mk (Local.tview lc_src) prom_src') lc_tgt'>>)
+  .
+  Proof.
+    inv STEPTGT. inv LCSRC. inv LCTGT. inv LOCAL.
+    hexploit sim_promise_forget; ss; eauto.
+
+
+      exists self' vw_src' prom_src' mem_src'
+             prom0 prom1 mem0 mem1 kind_src,
+        (<<FUTURE0: reserve_future_memory lc_src.(Local.promises) mem_src prom0 mem0>>) /\
+        (<<STEPSRC: Local.write_step (Local.mk vw_src prom0) sc mem0 loc from' to val releasedm released ord (Local.mk vw_src' prom1) sc mem1 kind_src>>) /\
+        (<<FUTURE1: reserve_future_memory prom1 mem1 prom_src' mem_src'>>) /\
+        (<<MEM: sim_memory (others \\2// self') mem_src' mem_tgt'>>) /\
+        (<<SIM: sim_local self' (Local.mk vw_src' prom_src') lc_tgt'>>)
+  .
+
+      exists lc_src' mem_src',
+        (<<FUTURE: reserve_fu
+
+           Local.promise_step lc_src mem_src loc from to msg lc_src' mem_src' kind>>) /\
+        (<<MEM: sim_memory (others \\2// self) (extra_others \\3// extra_self) mem_src' mem_tgt'>>) /\
+        (<<LOCAL: sim_local self extra_self lc_src' lc_tgt'>>)
+  .
+  Proof.
+    inv LOCAL. inv LCSRC. inv LCTGT. inv STEPTGT. ss.
+    hexploit sim_promise_normal; eauto. i. des.
+    exists (Local.mk tvw prom_src'), mem_src'. splits; eauto.
+  Qed.
+
+
+  Lemma sim_write_step_forget
+        others self extra_others extra_self lc_src lc_tgt sc mem_src mem_tgt
+        lc_tgt' sc' mem_tgt' loc from to val ord releasedm released kind
+        (NLOC: ~ L loc)
+        (STEPTGT: Local.write_step lc_tgt sc mem_tgt loc from to val releasedm released ord lc_tgt' sc' mem_tgt' kind)
+        (MEM: sim_memory (others \\2// self) (extra_others \\3// extra_self) mem_src mem_tgt)
+        (SCSRC: Memory.closed_timemap sc mem_src)
+        (SCTGT: Memory.closed_timemap sc mem_tgt)
+        (MEMSRC: Memory.closed mem_src)
+        (MEMTGT: Memory.closed mem_tgt)
+        (LOCALSRC: Local.wf lc_src mem_src)
+        (LOCALTGT: Local.wf lc_tgt mem_tgt)
+        (SIM: sim_local self extra_self lc_src lc_tgt)
+
+        (RELEASEDMCLOSED: Memory.closed_opt_view releasedm mem_src)
+        (RELEASEDMWF: View.opt_wf releasedm)
+    :
+      exists lc_src' mem_src',
+        (<<STEPSRC: Local.write_step lc_src sc mem_src loc from to val releasedm released ord lc_src' sc' mem_src' kind>>) /\
+        (<<MEM: sim_memory (others \\2// self) (extra_others \\3// extra_self) mem_src' mem_tgt'>>) /\
+        (<<SIM: sim_local self extra_self lc_src' lc_tgt'>>)
+  .
+  Proof.
 
 
 
@@ -2567,787 +2791,6 @@ Section SIM.
 
     Memory.write
 
-  Lemma promise_replace_write self loc from from' to prom0 mem0 val released
-        (LIN: L loc)
-        (* (SELF: self <2= promised prom0) *)
-        (LOC: forall from to msg (GET: Memory.get loc to prom0 = Some (from, msg)),
-            msg = Message.reserve)
-        (MLE0: Memory.le prom0 mem0)
-        (NBOT: Time.lt Time.bot to)
-        (PROMISED: self loc to)
-        (GET: Memory.get loc to prom0 = Some (from, Message.reserve))
-        (FROM: Time.lt from' to)
-        (EMPTY: forall ts (ITV: Interval.mem (from', from) ts), ~ covered loc ts mem0)
-        (VIEWWF: View.opt_wf released)
-        (MSGTO: Time.le (View.rlx (View.unwrap released) loc) to)
-    :
-      exists prom1 mem1 prom2 mem2 prom3 mem3,
-        (<<FUTURE01: reserve_future_memory prom0 mem0 prom1 mem1>>) /\
-        (<<WRITE: Memory.write prom1 mem1 loc from' to val released prom2 mem2 Memory.op_kind_add>>) /\
-        (<<FUTURE23: reserve_future_memory prom2 mem2 prom3 mem3>>) /\
-        (<<MEMSPEC: forall loc' ts',
-            Memory.get loc' ts' mem3 =
-            if loc_ts_eq_dec (loc', ts') (loc, to)
-            then Some (from', Message.concrete val released)
-            else Memory.get loc' ts' mem0>>) /\
-        (<<PROMSPEC: forall loc' ts',
-            Memory.get loc' ts' prom3 =
-            if loc_ts_eq_dec (loc', ts') (loc, to)
-            then None
-            else Memory.get loc' ts' prom0>>).
-  Proof.
-    hexploit promises_not_attached_replaces; eauto.
-    { econs; eauto. }
-    i. des.
-    hexploit (@Memory.remove_exists prom1 loc from to Message.reserve).
-    { hexploit (@UNCH01 loc to); eauto.
-      { i. refl. }
-      i. des. erewrite PROM. eauto. }
-    intros [prom2 REMOVEPROM].
-    hexploit Memory.remove_exists_le; eauto.
-    intros [mem2 REMOVEMEM].
-    assert (PROMISE0: Memory.promise prom1 mem1 loc from to Message.reserve prom2 mem2 Memory.op_kind_cancel).
-    { econs; eauto. }
-    hexploit (@Memory.add_exists mem2 loc from' to (Message.concrete val released)); eauto.
-
-    { ii. erewrite Memory.remove_o in GET2; eauto. des_ifs. guardH o.
-      hexploit (@Memory.get_disjoint loc from2 from to2 to).
-      { eapply GET2. }
-      { hexploit (@UNCH01 loc to).
-        { i. refl. }
-        i. des. rewrite MEM. eauto. }
-      i. ss. unguard. des; clarify.
-      eapply H; eauto. inv LHS. econs; ss.
-      destruct (Time.le_lt_dec x from); auto. exfalso.
-      hexploit memory_get_to_mon.
-      { eapply GET2. }
-      { hexploit (@UNCH01 loc to).
-        { i. refl. }
-        i. des. rewrite MEM. eauto. }
-      { inv RHS. ss. eapply TimeFacts.lt_le_lt; eauto. }
-      i. hexploit (@UNCH01 loc to2).
-      { i. left. auto. }
-      i. des. erewrite MEM in *. eapply (EMPTY x).
-      { econs; ss. }
-      { econs; eauto. }
-    }
-    { econs; eauto. }
-    intros [mem2' ADDMEM].
-    hexploit (@Memory.add_exists_le prom2 mem2 loc from' to (Message.concrete val released)); eauto.
-    { eapply promise_memory_le; eauto. }
-    intros [prom2' ADDPROM].
-
-    assert (PROMISE1: Memory.write prom2 mem2 loc from' to val released prom2 mem2' Memory.op_kind_add).
-    { econs; eauto.
-      - econs; eauto. i.
-        erewrite (@Memory.remove_o mem2) in GET0; eauto.
-        des_ifs. eauto.
-      - exploit Memory.remove_exists.
-        { eapply Memory.add_get0 in ADDPROM. des. eapply GET1. }
-        i. des.
-        exploit MemoryFacts.add_remove_eq; eauto. i. subst. auto.
-    }
-
-    hexploit (@RESTORE prom2 mem2'); eauto.
-    { i. erewrite (@Memory.add_o mem2'); eauto.
-      erewrite (@Memory.remove_o mem2); eauto.
-      erewrite (@Memory.remove_o prom2); eauto. des_ifs.
-      ss. des; clarify. exfalso. eapply Time.lt_strorder; eauto. }
-    { eapply write_memory_le; cycle 1; eauto.
-      eapply promise_memory_le; cycle 1; eauto. }
-    i. des.
-    exists prom2, mem2, prom2, mem2', prom3, mem3. splits; auto.
-    { eapply reserve_future_memory_trans; eauto. }
-    { i. destruct (classic (loc' = loc -> Time.lt to ts')).
-      - hexploit UNCHANGED; eauto. i. des. rewrite MEM. des_ifs.
-        ss. des; clarify. exfalso. eapply Time.lt_strorder; eauto.
-      - apply imply_to_and in H. des. clarify.
-        hexploit (@CHANGED ts'); eauto.
-        { destruct (Time.le_lt_dec ts' to); eauto. exfalso. auto. }
-        i. des. rewrite MEM.
-        erewrite (@Memory.add_o mem2' mem2); eauto.
-        erewrite (@Memory.remove_o mem2 mem1); eauto.
-        des_ifs. guardH o. hexploit (@UNCH01 loc ts'); eauto.
-        { i. destruct (Time.le_lt_dec ts' to); eauto. exfalso. auto. }
-        i. des; clarify.
-    }
-    { i. destruct (classic (loc' = loc -> Time.lt to ts')).
-      - hexploit UNCHANGED; eauto. i. des. rewrite PROM. des_ifs.
-        ss. des; clarify. exfalso. eapply Time.lt_strorder; eauto.
-      - apply imply_to_and in H. des. clarify.
-        hexploit (@CHANGED ts'); eauto.
-        { destruct (Time.le_lt_dec ts' to); eauto. exfalso. auto. }
-        i. des. rewrite PROM.
-        erewrite (@Memory.remove_o prom2 prom1); eauto.
-        des_ifs. guardH o. hexploit (@UNCH01 loc ts'); eauto.
-        { i. destruct (Time.le_lt_dec ts' to); eauto. exfalso. auto. }
-        i. des; clarify.
-    }
-  Qed.
-
-
-
-
-  Lemma promises_not_attached_replaces self loc ts prom0 mem0
-        (LIN: L loc)
-        (ATTACHED: promises_not_attached self (promised prom0) mem0)
-        (* (SELF: self <2= promised prom0) *)
-        (LOC: forall from to msg (GET: Memory.get loc to prom0 = Some (from, msg)),
-            msg = Message.reserve)
-        (MLE0: Memory.le prom0 mem0)
-        (NBOT: Time.lt Time.bot ts)
-        (* (SELF: self loc ts) *)
-        (PROMISED: promised prom0 loc ts)
-    :
-      exists prom1 mem1,
-        (<<FUTURE01: reserve_future_memory prom0 mem0 prom1 mem1>>) /\
-        (<<UNCH01: forall loc' to (TS: loc' = loc -> Time.le to ts),
-            (<<MEM: Memory.get loc' to mem1 = Memory.get loc' to mem0>>) /\
-            (<<PROM: Memory.get loc' to prom1 = Memory.get loc' to prom0>>)>>) /\
-
-        (<<ATTACH: forall to msg (SELF: self loc ts) (GET: Memory.get loc to mem1 = Some (ts, msg)), False>>) /\
-        (* (<<ATTACH: forall to msg (GET: Memory.get loc to mem1 = Some (ts, msg)), False>>) /\ *)
-
-        (<<MLE1: Memory.le prom1 mem1>>) /\
-
-        (<<RESTORE:
-           forall prom2 mem2
-                  (UNCH12: forall loc' to (TS: loc' = loc -> Time.lt ts to),
-                      (<<MEM: Memory.get loc' to mem2 = Memory.get loc' to mem1>>) /\
-                      (<<PROM: Memory.get loc' to prom2 = Memory.get loc' to prom1>>))
-                  (MLE2: Memory.le prom2 mem2)
-           ,
-           exists prom3 mem3,
-             (<<FUTURE23: reserve_future_memory prom2 mem2 prom3 mem3>>) /\
-             (<<UNCHANGED: forall loc' to (TS: loc' = loc -> Time.lt ts to),
-                 (<<MEM: Memory.get loc' to mem3 = Memory.get loc' to mem0>>) /\
-                 (<<PROM: Memory.get loc' to prom3 = Memory.get loc' to prom0>>)>>) /\
-             (<<CHANGED: forall to (TS: Time.le to ts),
-                 (<<MEM: Memory.get loc to mem3 = Memory.get loc to mem2>>) /\
-                 (<<PROM: Memory.get loc to prom3 = Memory.get loc to prom2>>)>>) /\
-             (<<MLE3: Memory.le prom3 mem3>>)
-               >>).
-  Proof.
-    destruct (classic (self loc ts)) as [SELF|NSELF]; cycle 1.
-    { exists prom0, mem0. splits; eauto. i. esplits; eauto. }
-    destruct (classic (exists to msg, <<GET: Memory.get loc to mem0 = Some (ts, msg)>>)); cycle 1.
-    { exists prom0, mem0. splits; eauto. i. esplits; eauto. }
-    des. exploit ATTACHED; eauto. i. inv x. destruct msg0 as [from msg0].
-    dup GET0. apply MLE0 in GET1. clarify.
-    exploit LOC; eauto. i. clarify.
-
-    assert (TSTO: Time.lt ts to).
-    { eapply memory_get_ts_strong in GET0. des; auto. clarify. }
-
-    exploit Memory.remove_exists.
-    { eapply GET0. }
-    intros [prom1 REMOVEPROM].
-    exploit Memory.remove_exists_le; eauto.
-    intros [mem1 REMOVEMEM].
-
-    assert (REMOVE: Memory.promise prom0 mem0 loc ts to Message.reserve prom1 mem1 Memory.op_kind_cancel).
-    { econs; eauto. }
-    exists prom1, mem1. splits; eauto.
-    { i. erewrite (@Memory.remove_o mem1); eauto.
-      erewrite (@Memory.remove_o prom1); eauto. des_ifs.
-      ss. des; clarify.
-      exfalso. eapply Time.lt_strorder. eapply TimeFacts.lt_le_lt; eauto.
-    }
-    { i. erewrite Memory.remove_o in GET; eauto. des_ifs. ss. des; clarify.
-      exploit memory_get_from_inj.
-      { eapply GET. }
-      { eapply GET1. }
-      i. des; clarify.
-      { eapply Time.lt_strorder; eauto. }
-      { eapply Time.lt_strorder; eauto. }
-    }
-    { eapply promise_memory_le; eauto. }
-    { i. hexploit (@Memory.add_exists mem2 loc ts to Message.reserve).
-      { ii. hexploit (@UNCH12 loc to2).
-        { i. inv LHS. inv RHS. ss. eapply TimeFacts.lt_le_lt; eauto. }
-        i. des. rewrite H in *.
-        erewrite (@Memory.remove_o mem1) in GET2; eauto. des_ifs. guardH o.
-        exploit Memory.get_disjoint.
-        { eapply GET2. }
-        { eapply GET1. }
-        i. des; clarify.
-        - ss. unguard. des; clarify.
-        - eapply x1; eauto.
-      }
-      { auto. }
-      { econs. }
-      intros [mem3 ADDMEM].
-      hexploit (Memory.add_exists_le); eauto.
-      intros [prom3 ADDPROM].
-
-      assert (ADD: Memory.promise prom2 mem2 loc ts to Message.reserve prom3 mem3 Memory.op_kind_add).
-      { econs; eauto. i. clarify. }
-
-      exists prom3, mem3. splits; auto.
-      { eapply reserve_future_memory_trans; eauto. }
-
-      { i. exploit UNCH12; eauto. i. des.
-        erewrite (@Memory.add_o mem3); eauto.
-        erewrite (@Memory.add_o prom3); eauto.
-        erewrite x. erewrite x0.
-        erewrite (@Memory.remove_o mem1); eauto.
-        erewrite (@Memory.remove_o prom1); eauto. des_ifs.
-        ss. des; clarify. }
-      { i. erewrite (@Memory.add_o mem3); eauto.
-        erewrite (@Memory.add_o prom3); eauto. des_ifs.
-        ss. des; clarify.
-        exfalso. eapply Time.lt_strorder.
-        eapply (@TimeFacts.le_lt_lt to ts); eauto. }
-      { eapply promise_memory_le; eauto. }
-    }
-  Qed.
-
-  Lemma promises_not_attached_replace_add self loc from from' to prom0 mem0
-        (LIN: L loc)
-        (ATTACHED: promises_not_attached self (promised prom0) mem0)
-        (LOC: forall from to msg (GET: Memory.get loc to prom0 = Some (from, msg)),
-            msg = Message.reserve)
-        (MLE0: Memory.le prom0 mem0)
-        (NBOT: Time.lt Time.bot to)
-        (* (PROMISED: self loc to) *)
-        (GET: Memory.get loc to prom0 = Some (from, Message.reserve))
-        (FROM: Time.lt from' to)
-        (EMPTY: forall ts (ITV: Interval.mem (from', from) ts), ~ covered loc ts mem0)
-    :
-      exists prom1 mem1,
-        (<<FUTURE01: reserve_future_memory prom0 mem0 prom1 mem1>>) /\
-        (<<MEMSPEC: forall loc' ts',
-            Memory.get loc' ts' mem1 =
-            if loc_ts_eq_dec (loc', ts') (loc, to)
-            then Some (from', Message.reserve)
-            else Memory.get loc' ts' mem0>>) /\
-        (<<PROMSPEC: forall loc' ts',
-            Memory.get loc' ts' prom1 =
-            if loc_ts_eq_dec (loc', ts') (loc, to)
-            then Some (from', Message.reserve)
-            else Memory.get loc' ts' prom0>>).
-  Proof.
-    hexploit promises_not_attached_replaces; eauto.
-    { econs; eauto. }
-    i. des.
-    hexploit (@Memory.remove_exists prom1 loc from to Message.reserve).
-    { hexploit (@UNCH01 loc to); eauto.
-      { i. refl. }
-      i. des. erewrite PROM. eauto. }
-    intros [prom2 REMOVEPROM].
-    hexploit Memory.remove_exists_le; eauto.
-    intros [mem2 REMOVEMEM].
-    assert (PROMISE0: Memory.promise prom1 mem1 loc from to Message.reserve prom2 mem2 Memory.op_kind_cancel).
-    { econs; eauto. }
-    hexploit (@Memory.add_exists mem2 loc from' to Message.reserve); eauto.
-
-    { ii. erewrite Memory.remove_o in GET2; eauto. des_ifs. guardH o.
-      hexploit (@Memory.get_disjoint loc from2 from to2 to).
-      { eapply GET2. }
-      { hexploit (@UNCH01 loc to).
-        { i. refl. }
-        i. des. rewrite MEM. eauto. }
-      i. ss. unguard. des; clarify.
-      eapply H; eauto. inv LHS. econs; ss.
-      destruct (Time.le_lt_dec x from); auto. exfalso.
-      hexploit memory_get_to_mon.
-      { eapply GET2. }
-      { hexploit (@UNCH01 loc to).
-        { i. refl. }
-        i. des. rewrite MEM. eauto. }
-      { inv RHS. ss. eapply TimeFacts.lt_le_lt; eauto. }
-      i. hexploit (@UNCH01 loc to2).
-      { i. left. auto. }
-      i. des. erewrite MEM in *. eapply (EMPTY x).
-      { econs; ss. }
-      { econs; eauto. }
-    }
-    { econs. }
-    intros [mem2' ADDMEM].
-    hexploit (@Memory.add_exists_le prom2 mem2 loc from' to Message.reserve); eauto.
-    { eapply promise_memory_le; eauto. }
-    intros [prom2' ADDPROM].
-    assert (PROMISE1: Memory.promise prom2 mem2 loc from' to Message.reserve prom2' mem2' Memory.op_kind_add).
-    { econs; eauto. i. clarify. }
-    hexploit (@RESTORE prom2' mem2'); eauto.
-    { i. erewrite (@Memory.add_o mem2'); eauto.
-      erewrite (@Memory.add_o prom2'); eauto.
-      erewrite (@Memory.remove_o mem2); eauto.
-      erewrite (@Memory.remove_o prom2); eauto. des_ifs.
-      ss. des; clarify. exfalso. eapply Time.lt_strorder; eauto. }
-    { eapply promise_memory_le; cycle 1; eauto.
-      eapply promise_memory_le; cycle 1; eauto. }
-    i. des. exists prom3, mem3. splits; auto.
-    { eapply reserve_future_memory_trans; eauto. }
-    { i. destruct (classic (loc' = loc -> Time.lt to ts')).
-      - hexploit UNCHANGED; eauto. i. des. rewrite MEM. des_ifs.
-        ss. des; clarify. exfalso. eapply Time.lt_strorder; eauto.
-      - apply imply_to_and in H. des. clarify.
-        hexploit (@CHANGED ts'); eauto.
-        { destruct (Time.le_lt_dec ts' to); eauto. exfalso. auto. }
-        i. des. rewrite MEM.
-        erewrite (@Memory.add_o mem2' mem2); eauto.
-        erewrite (@Memory.remove_o mem2 mem1); eauto.
-        des_ifs. guardH o. hexploit (@UNCH01 loc ts'); eauto.
-        { i. destruct (Time.le_lt_dec ts' to); eauto. exfalso. auto. }
-        i. des; clarify.
-    }
-    { i. destruct (classic (loc' = loc -> Time.lt to ts')).
-      - hexploit UNCHANGED; eauto. i. des. rewrite PROM. des_ifs.
-        ss. des; clarify. exfalso. eapply Time.lt_strorder; eauto.
-      - apply imply_to_and in H. des. clarify.
-        hexploit (@CHANGED ts'); eauto.
-        { destruct (Time.le_lt_dec ts' to); eauto. exfalso. auto. }
-        i. des. rewrite PROM.
-        erewrite (@Memory.add_o prom2' prom2); eauto.
-        erewrite (@Memory.remove_o prom2 prom1); eauto.
-        des_ifs. guardH o. hexploit (@UNCH01 loc ts'); eauto.
-        { i. destruct (Time.le_lt_dec ts' to); eauto. exfalso. auto. }
-        i. des; clarify.
-    }
-  Qed.
-
-  Lemma sim_promise_weak_stengthen others self prom_src prom_tgt mem_src mem_tgt
-        (MEM: sim_memory (others \\2// self) mem_src mem_tgt)
-        (MLETGT: Memory.le prom_tgt mem_tgt)
-        (MLESRC: Memory.le prom_src mem_src)
-        (FIN: Memory.finite prom_src)
-        (BOTNONE: Memory.bot_none prom_src)
-        (PROM: sim_promise self prom_src prom_tgt)
-        (PROMATTACH: promises_not_attached self (promised prom_src) mem_src)
-        (* (SELF: self <2= promised prom_src) *)
-        (EXCLUSIVE: forall loc' ts' (SELF: self loc' ts') (OTHER: others loc' ts'), False)
-    :
-      exists prom_src' mem_src',
-        (<<FUTURE: reserve_future_memory prom_src mem_src prom_src' mem_src'>>) /\
-        (<<MEM: sim_memory (others \\2// self) mem_src' mem_tgt>>) /\
-        (<<ATTACHEDLE: not_attached_le others mem_src mem_src'>>) /\
-        (<<PROMATTACH: promises_not_attached self (promised prom_src') mem_src'>>) /\
-        (<<PROM: sim_promise_strong
-                   self (concrete_promised mem_src' \\2// self)
-                   (* (fun loc' ts' => concrete_promise *)
-                   (*    concrete_promised prom_src' loc' ts' /\ *)
-                   (*    ~ others loc' ts' *)
-                   (* ) *)
-                   prom_src' prom_tgt>>).
-  Proof.
-    exploit sim_promise_weak_list_exists; eauto. i. des.
-    clear PROM. ginduction l.
-    { i. exists prom_src, mem_src. splits; auto.
-      - refl.
-      - eapply sim_promise_list_nil; eauto. }
-    i. destruct a as [loc ts].
-    dup SIM. specialize (SIM0 loc ts). des.
-    { exploit IHl; eauto. ii.
-      destruct (loc_ts_eq_dec (loc0, ts0) (loc, ts)).
-      - ss. des; clarify. left. auto.
-      - specialize (SIM loc0 ts0). ss. des; auto; clarify. }
-
-    clear LIN.
-
-    destruct (Memory.get loc ts prom_src) as [[from_src [val released|]]|] eqn:GETSRC; cycle 2.
-    { inv WEAK. exploit IHl; eauto. ii.
-      specialize (SIM loc0 ts0). ss. des; auto; clarify.
-      left. rewrite <- H. rewrite GETSRC. econs; eauto. }
-    { inv WEAK. exploit IHl; eauto. ii.
-      specialize (SIM loc0 ts0). ss. des; auto; clarify.
-      left. rewrite <- H. rewrite GETSRC. econs; eauto. }
-    assert (exists from_tgt msg, <<GETTGT: Memory.get loc ts prom_tgt = Some (from_tgt, msg)>>).
-    { inv WEAK; eauto. } des. rewrite GETTGT in *.
-
-    destruct (classic ((concrete_promised mem_src \\2// self) loc from_tgt)) as [OTHER|NOTHER]; cycle 1.
-    { exploit IHl; eauto. ii.
-      specialize (SIM loc0 ts0). ss. des; auto; clarify.
-      left. rewrite GETTGT. rewrite GETSRC. inv WEAK.
-      - econs 2; eauto.
-      - econs 3; eauto. clarify.
-      - econs 4; eauto. clarify. }
-    guardH OTHER.
-
-    assert (NBOT: Time.lt Time.bot ts).
-    { destruct (Time.le_lt_dec ts Time.bot); auto. destruct l0.
-      - exfalso. eapply Time.lt_strorder.
-        eapply TimeFacts.lt_le_lt; eauto. eapply Time.bot_spec.
-      - inv H. erewrite BOTNONE in GETSRC. clarify. }
-
-    destruct (classic (L loc)) as [LOC|NLOC]; cycle 1.
-    { hexploit (@IHl others self prom_src prom_tgt mem_src mem_tgt); eauto.
-      ii. specialize (SIM loc0 ts0). ss. des; eauto. clarify.
-      left. inv WEAK; eauto.
-      - rewrite GETSRC. rewrite GETTGT. econs 2; eauto.
-      - rewrite GETSRC. rewrite GETTGT. econs 3; eauto. i. clarify.
-      - rewrite GETSRC. rewrite GETTGT. econs 4; eauto. i. clarify. }
-
-    exploit promises_not_attached_replace_add.
-    { eauto. }
-    { eauto. }
-    { ii. specialize (SIM loc to). rewrite GET in *. des.
-      - inv NORMAL; eauto; try by (exfalso; eauto).
-      - inv WEAK0; eauto; try by (exfalso; eauto). }
-    { eauto. }
-    { eauto. }
-    { eauto. }
-    { instantiate (1:=from_tgt).
-      apply memory_get_ts_strong in GETTGT. des; clarify. }
-    { ii. inv H. specialize (MEM loc to). rewrite GET in MEM.
-      inv MEM; clarify.
-      - exploit Memory.get_disjoint.
-        { symmetry. apply H. }
-        { eapply MLETGT. eapply GETTGT. }
-        i. des; clarify.
-        + eapply MLESRC in GETSRC. clarify.
-          inv ITV. inv ITV0. ss. clear - TO FROM1.
-          eapply Time.lt_strorder. eapply TimeFacts.le_lt_lt; eauto.
-        + eapply x0.
-          * instantiate (1:=ts0). econs; ss.
-            { inv ITV0. eapply TimeFacts.le_lt_lt; eauto. }
-            { inv ITV0. ss. }
-          * inv ITV. econs; ss. etrans; eauto.
-            eapply memory_get_ts_le; eauto.
-      - guardH PROM. exploit Memory.get_disjoint.
-        { symmetry. apply H. }
-        { eapply MLETGT. eapply GETTGT. }
-        i. des; clarify.
-        + eapply MLESRC in GETSRC. clarify.
-          inv ITV. inv ITV0. ss. clear - TO FROM1.
-          eapply Time.lt_strorder. eapply TimeFacts.le_lt_lt; eauto.
-        + eapply x0.
-          * instantiate (1:=ts0). econs; ss.
-            { inv ITV0. eapply TimeFacts.le_lt_lt; eauto. }
-            { inv ITV0. ss. }
-          * inv ITV. econs; ss. etrans; eauto.
-            eapply memory_get_ts_le; eauto.
-    }
-    i. des.
-    assert (PROMISEDSAME: promised prom1 = promised prom_src).
-    { extensionality loc'. extensionality ts'.
-      apply Coq.Logic.PropExtensionality.propositional_extensionality.
-      split; i.
-      - inv H. erewrite PROMSPEC in GET. des_ifs.
-        + ss. des; clarify. econs; eauto.
-        + econs; eauto.
-      - inv H. specialize (PROMSPEC loc' ts'). des_ifs.
-        + ss. des; clarify. econs; eauto.
-        + erewrite <- PROMSPEC in *. econs; eauto. }
-    assert (CONCRETESAME: concrete_promised mem1 = concrete_promised mem_src).
-    { extensionality loc'. extensionality ts'.
-      apply Coq.Logic.PropExtensionality.propositional_extensionality.
-      split; i.
-      - inv H. erewrite MEMSPEC in GET. des_ifs. econs; eauto.
-      - inv H. specialize (MEMSPEC loc' ts'). des_ifs.
-        + ss. des; clarify. apply MLESRC in GETSRC. clarify.
-        + erewrite <- MEMSPEC in *. econs; eauto. }
-
-    assert (PROMISEDSAMEMEM: promised mem1 = promised mem_src).
-    { extensionality loc'. extensionality ts'.
-      apply Coq.Logic.PropExtensionality.propositional_extensionality.
-      split; i.
-      - inv H. erewrite MEMSPEC in GET. des_ifs.
-        + ss. des; clarify. econs; eauto.
-        + econs; eauto.
-      - inv H. specialize (MEMSPEC loc' ts'). des_ifs.
-        + ss. des; clarify. econs; eauto.
-        + erewrite <- MEMSPEC in *. econs; eauto. }
-
-    hexploit (@IHl others self prom1 prom_tgt mem1 mem_tgt); eauto.
-    { ii.
-      dup MEM. specialize (MEM0 loc0 ts0). erewrite MEMSPEC. des_ifs.
-      - ss. des; clarify. apply MLETGT in GETTGT. rewrite GETTGT.
-        rewrite GETTGT in *. apply MLESRC in GETSRC. rewrite GETSRC in *.
-        inv MEM0; eauto.
-        + econs 2; eauto. refl.
-        + econs 3; eauto. refl.
-    }
-    { eapply reserve_future_memory_le; eauto. }
-    { eapply reserve_future_memory_finite; eauto. }
-    { eapply reserve_future_memory_bot_none; eauto. }
-    { ii. rewrite MEMSPEC in GET.
-      erewrite PROMISEDSAME. des_ifs.
-      - ss. des; clarify. econs; eauto.
-      - exploit PROMATTACH; eauto. }
-    { ii. erewrite PROMSPEC. des_ifs.
-      - left. ss. des. clarify. erewrite GETTGT. inv WEAK; eauto.
-      - guardH o. specialize (SIM loc0 ts0).
-        ss. rewrite CONCRETESAME. des; eauto.
-        unguard. des; clarify. }
-    i. des. exists prom_src', mem_src'. splits; auto.
-    - eapply reserve_future_memory_trans; eauto.
-    - etrans; eauto. ii.
-      erewrite MEMSPEC in GET. des_ifs.
-      + ss. des; clarify. exfalso.
-        specialize (MEM loc from). unguard. des.
-        * inv OTHER. erewrite GET in MEM. inv MEM. eauto.
-        * eauto.
-      + eauto.
-  Qed.
-
-  Lemma promises_not_attached_replace_write self loc from from' to prom0 mem0 val released
-        (LIN: L loc)
-        (ATTACHED: promises_not_attached self (promised prom0) mem0)
-        (* (SELF: self <2= promised prom0) *)
-        (LOC: forall from to msg (GET: Memory.get loc to prom0 = Some (from, msg)),
-            msg = Message.reserve)
-        (MLE0: Memory.le prom0 mem0)
-        (NBOT: Time.lt Time.bot to)
-        (PROMISED: self loc to)
-        (GET: Memory.get loc to prom0 = Some (from, Message.reserve))
-        (FROM: Time.lt from' to)
-        (EMPTY: forall ts (ITV: Interval.mem (from', from) ts), ~ covered loc ts mem0)
-        (VIEWWF: View.opt_wf released)
-        (MSGTO: Time.le (View.rlx (View.unwrap released) loc) to)
-    :
-      exists prom1 mem1 prom2 mem2 prom3 mem3,
-        (<<FUTURE01: reserve_future_memory prom0 mem0 prom1 mem1>>) /\
-        (<<WRITE: Memory.write prom1 mem1 loc from' to val released prom2 mem2 Memory.op_kind_add>>) /\
-        (<<FUTURE23: reserve_future_memory prom2 mem2 prom3 mem3>>) /\
-        (<<MEMSPEC: forall loc' ts',
-            Memory.get loc' ts' mem3 =
-            if loc_ts_eq_dec (loc', ts') (loc, to)
-            then Some (from', Message.concrete val released)
-            else Memory.get loc' ts' mem0>>) /\
-        (<<PROMSPEC: forall loc' ts',
-            Memory.get loc' ts' prom3 =
-            if loc_ts_eq_dec (loc', ts') (loc, to)
-            then None
-            else Memory.get loc' ts' prom0>>).
-  Proof.
-    hexploit promises_not_attached_replaces; eauto.
-    { econs; eauto. }
-    i. des.
-    hexploit (@Memory.remove_exists prom1 loc from to Message.reserve).
-    { hexploit (@UNCH01 loc to); eauto.
-      { i. refl. }
-      i. des. erewrite PROM. eauto. }
-    intros [prom2 REMOVEPROM].
-    hexploit Memory.remove_exists_le; eauto.
-    intros [mem2 REMOVEMEM].
-    assert (PROMISE0: Memory.promise prom1 mem1 loc from to Message.reserve prom2 mem2 Memory.op_kind_cancel).
-    { econs; eauto. }
-    hexploit (@Memory.add_exists mem2 loc from' to (Message.concrete val released)); eauto.
-
-    { ii. erewrite Memory.remove_o in GET2; eauto. des_ifs. guardH o.
-      hexploit (@Memory.get_disjoint loc from2 from to2 to).
-      { eapply GET2. }
-      { hexploit (@UNCH01 loc to).
-        { i. refl. }
-        i. des. rewrite MEM. eauto. }
-      i. ss. unguard. des; clarify.
-      eapply H; eauto. inv LHS. econs; ss.
-      destruct (Time.le_lt_dec x from); auto. exfalso.
-      hexploit memory_get_to_mon.
-      { eapply GET2. }
-      { hexploit (@UNCH01 loc to).
-        { i. refl. }
-        i. des. rewrite MEM. eauto. }
-      { inv RHS. ss. eapply TimeFacts.lt_le_lt; eauto. }
-      i. hexploit (@UNCH01 loc to2).
-      { i. left. auto. }
-      i. des. erewrite MEM in *. eapply (EMPTY x).
-      { econs; ss. }
-      { econs; eauto. }
-    }
-    { econs; eauto. }
-    intros [mem2' ADDMEM].
-    hexploit (@Memory.add_exists_le prom2 mem2 loc from' to (Message.concrete val released)); eauto.
-    { eapply promise_memory_le; eauto. }
-    intros [prom2' ADDPROM].
-
-    assert (PROMISE1: Memory.write prom2 mem2 loc from' to val released prom2 mem2' Memory.op_kind_add).
-    { econs; eauto.
-      - econs; eauto. i.
-        erewrite (@Memory.remove_o mem2) in GET0; eauto.
-        des_ifs. eauto.
-      - exploit Memory.remove_exists.
-        { eapply Memory.add_get0 in ADDPROM. des. eapply GET1. }
-        i. des.
-        exploit MemoryFacts.add_remove_eq; eauto. i. subst. auto.
-    }
-
-    hexploit (@RESTORE prom2 mem2'); eauto.
-    { i. erewrite (@Memory.add_o mem2'); eauto.
-      erewrite (@Memory.remove_o mem2); eauto.
-      erewrite (@Memory.remove_o prom2); eauto. des_ifs.
-      ss. des; clarify. exfalso. eapply Time.lt_strorder; eauto. }
-    { eapply write_memory_le; cycle 1; eauto.
-      eapply promise_memory_le; cycle 1; eauto. }
-    i. des.
-    exists prom2, mem2, prom2, mem2', prom3, mem3. splits; auto.
-    { eapply reserve_future_memory_trans; eauto. }
-    { i. destruct (classic (loc' = loc -> Time.lt to ts')).
-      - hexploit UNCHANGED; eauto. i. des. rewrite MEM. des_ifs.
-        ss. des; clarify. exfalso. eapply Time.lt_strorder; eauto.
-      - apply imply_to_and in H. des. clarify.
-        hexploit (@CHANGED ts'); eauto.
-        { destruct (Time.le_lt_dec ts' to); eauto. exfalso. auto. }
-        i. des. rewrite MEM.
-        erewrite (@Memory.add_o mem2' mem2); eauto.
-        erewrite (@Memory.remove_o mem2 mem1); eauto.
-        des_ifs. guardH o. hexploit (@UNCH01 loc ts'); eauto.
-        { i. destruct (Time.le_lt_dec ts' to); eauto. exfalso. auto. }
-        i. des; clarify.
-    }
-    { i. destruct (classic (loc' = loc -> Time.lt to ts')).
-      - hexploit UNCHANGED; eauto. i. des. rewrite PROM. des_ifs.
-        ss. des; clarify. exfalso. eapply Time.lt_strorder; eauto.
-      - apply imply_to_and in H. des. clarify.
-        hexploit (@CHANGED ts'); eauto.
-        { destruct (Time.le_lt_dec ts' to); eauto. exfalso. auto. }
-        i. des. rewrite PROM.
-        erewrite (@Memory.remove_o prom2 prom1); eauto.
-        des_ifs. guardH o. hexploit (@UNCH01 loc ts'); eauto.
-        { i. destruct (Time.le_lt_dec ts' to); eauto. exfalso. auto. }
-        i. des; clarify.
-    }
-  Qed.
-
-
-  Lemma promises_not_attached_replace_split self loc from from' to' to prom0 mem0
-        (LIN: L loc)
-        (ATTACHED: promises_not_attached self (promised prom0) mem0)
-        (* (SELF: self <2= promised prom0) *)
-        (* (PROMISED: self loc to) *)
-        (LOC: forall from to msg (GET: Memory.get loc to prom0 = Some (from, msg)),
-            msg = Message.reserve)
-        (MLE0: Memory.le prom0 mem0)
-        (NBOT: Time.lt Time.bot to)
-        (GET: Memory.get loc to prom0 = Some (from, Message.reserve))
-        (FROM: Time.lt from' to')
-        (TO: Time.lt to' to)
-        (EMPTY: forall ts (ITV: Interval.mem (from', from) ts), ~ covered loc ts mem0)
-    :
-      exists prom1 mem1,
-        (<<FUTURE01: reserve_future_memory prom0 mem0 prom1 mem1>>) /\
-        (<<MEMSPEC: forall loc' ts',
-            Memory.get loc' ts' mem1 =
-            if loc_ts_eq_dec (loc', ts') (loc, to')
-            then Some (from', Message.reserve)
-            else if loc_ts_eq_dec (loc', ts') (loc, to)
-                 then Some (to', Message.reserve)
-                 else Memory.get loc' ts' mem0>>) /\
-        (<<PROMSPEC: forall loc' ts',
-            Memory.get loc' ts' prom1 =
-            if loc_ts_eq_dec (loc', ts') (loc, to')
-            then Some (from', Message.reserve)
-            else if loc_ts_eq_dec (loc', ts') (loc, to)
-                 then Some (to', Message.reserve)
-                 else Memory.get loc' ts' prom0>>).
-  Proof.
-    hexploit promises_not_attached_replaces; eauto.
-    { econs; eauto. }
-    i. des.
-    hexploit (@Memory.remove_exists prom1 loc from to Message.reserve).
-    { hexploit (@UNCH01 loc to); eauto.
-      { i. refl. }
-      i. des. erewrite PROM. eauto. }
-    intros [prom2 REMOVEPROM].
-    hexploit Memory.remove_exists_le; eauto.
-    intros [mem2 REMOVEMEM].
-    assert (PROMISE0: Memory.promise prom1 mem1 loc from to Message.reserve prom2 mem2 Memory.op_kind_cancel).
-    { econs; eauto. }
-    assert (DISJOINT: forall (to2 from2 : Time.t) (msg2 : Message.t)
-                             (GET2: Memory.get loc to2 mem2 = Some (from2, msg2)),
-               Interval.disjoint (from', to) (from2, to2)).
-    { ii. erewrite Memory.remove_o in GET2; eauto. des_ifs. guardH o.
-      hexploit (@Memory.get_disjoint loc from2 from to2 to).
-      { eapply GET2. }
-      { hexploit (@UNCH01 loc to).
-        { i. refl. }
-        i. des. rewrite MEM. eauto. }
-      i. ss. unguard. des; clarify.
-      eapply H; eauto. inv LHS. econs; ss.
-      destruct (Time.le_lt_dec x from); auto. exfalso.
-      hexploit memory_get_to_mon.
-      { eapply GET2. }
-      { hexploit (@UNCH01 loc to).
-        { i. refl. }
-        i. des. rewrite MEM. eauto. }
-      { inv RHS. ss. eapply TimeFacts.lt_le_lt; eauto. }
-      i. hexploit (@UNCH01 loc to2).
-      { i. left. auto. }
-      i. des. erewrite MEM in *. eapply (EMPTY x).
-      { econs; ss. }
-      { econs; eauto. }
-    }
-
-    hexploit (@Memory.add_exists mem2 loc from' to' Message.reserve); eauto.
-    { ii. eapply DISJOINT; eauto. inv LHS. econs; ss.
-      etrans; eauto. left. auto. }
-    { econs. }
-    intros [mem2' ADDMEM0].
-    hexploit (@Memory.add_exists_le prom2 mem2 loc from' to' Message.reserve); eauto.
-    { eapply promise_memory_le; eauto. }
-    intros [prom2' ADDPROM0].
-    assert (PROMISE1: Memory.promise prom2 mem2 loc from' to' Message.reserve prom2' mem2' Memory.op_kind_add).
-    { econs; eauto. i. clarify. }
-
-    hexploit (@Memory.add_exists mem2' loc to' to Message.reserve); eauto.
-    { ii. erewrite Memory.add_o in GET2; eauto. des_ifs.
-      - ss. des; clarify. inv LHS. inv RHS. ss.
-        eapply Time.lt_strorder. eapply TimeFacts.le_lt_lt; eauto.
-      - guardH o. eapply DISJOINT; eauto. inv LHS. econs; ss.
-        etrans; eauto. }
-    { econs. }
-    intros [mem2'' ADDMEM1].
-    hexploit (@Memory.add_exists_le prom2' mem2' loc to' to Message.reserve); eauto.
-    { eapply promise_memory_le; cycle 1; eauto.
-      eapply promise_memory_le; cycle 1; eauto. }
-    intros [prom2'' ADDPROM1].
-
-    assert (PROMISE2: Memory.promise prom2' mem2' loc to' to Message.reserve prom2'' mem2'' Memory.op_kind_add).
-    { econs; eauto. i. clarify. }
-    hexploit (@RESTORE prom2'' mem2''); eauto.
-    { i. erewrite (@Memory.add_o mem2''); eauto.
-      erewrite (@Memory.add_o prom2''); eauto.
-      erewrite (@Memory.add_o mem2'); eauto.
-      erewrite (@Memory.add_o prom2'); eauto.
-      erewrite (@Memory.remove_o mem2); eauto.
-      erewrite (@Memory.remove_o prom2); eauto. des_ifs.
-      - ss. des; clarify. exfalso. eapply Time.lt_strorder; eauto.
-      - guardH o. ss. des; clarify. exfalso.
-        eapply Time.lt_strorder. etrans; eauto.
-    }
-    { eapply promise_memory_le; cycle 1; eauto.
-      eapply promise_memory_le; cycle 1; eauto.
-      eapply promise_memory_le; cycle 1; eauto. }
-    i. des. exists prom3, mem3. splits; auto.
-    { eapply reserve_future_memory_trans; eauto. }
-    { i. destruct (classic (loc' = loc -> Time.lt to ts')).
-      - hexploit UNCHANGED; eauto. i. des. rewrite MEM. des_ifs.
-        + ss. des; clarify. exfalso. eapply Time.lt_strorder; eauto.
-        + ss. des; clarify. exfalso. eapply Time.lt_strorder; eauto.
-      - apply imply_to_and in H. des. clarify.
-        hexploit (@CHANGED ts'); eauto.
-        { destruct (Time.le_lt_dec ts' to); eauto. exfalso. auto. }
-        i. des. rewrite MEM.
-        erewrite (@Memory.add_o mem2'' mem2'); eauto.
-        erewrite (@Memory.add_o mem2' mem2); eauto.
-        erewrite (@Memory.remove_o mem2 mem1); eauto.
-        des_ifs.
-        + ss. des; clarify.
-        + guardH o. guardH o0. hexploit (@UNCH01 loc ts'); eauto.
-          { i. destruct (Time.le_lt_dec ts' to); eauto. exfalso. auto. }
-          i. des; clarify.
-    }
-    { i. destruct (classic (loc' = loc -> Time.lt to ts')).
-      - hexploit UNCHANGED; eauto. i. des. rewrite PROM. des_ifs.
-        + ss. des; clarify. exfalso. eapply Time.lt_strorder; eauto.
-        + ss. des; clarify. exfalso. eapply Time.lt_strorder; eauto.
-      - apply imply_to_and in H. des. clarify.
-        hexploit (@CHANGED ts'); eauto.
-        { destruct (Time.le_lt_dec ts' to); eauto. exfalso. auto. }
-        i. des. rewrite PROM.
-        erewrite (@Memory.add_o prom2'' prom2'); eauto.
-        erewrite (@Memory.add_o prom2' prom2); eauto.
-        erewrite (@Memory.remove_o prom2 prom1); eauto.
-        des_ifs.
-        + ss. des; clarify.
-        + guardH o. hexploit (@UNCH01 loc ts'); eauto.
-          { i. destruct (Time.le_lt_dec ts' to); eauto. exfalso. auto. }
-          i. des; clarify.
-    }
-  Qed.
-
-
   Lemma sim_promise_step_forget others self mem_src mem_tgt prom_src prom_tgt
         loc from to msg_tgt prom_tgt' mem_tgt' kind_tgt
         (LOC: L loc)
@@ -3358,7 +2801,6 @@ Section SIM.
         (WFSRC: Memory.le prom_src mem_src)
         (WFTGT: Memory.le prom_tgt mem_tgt)
         (PROMISE: sim_promise self prom_src prom_tgt)
-        (PROMATTACH: promises_not_attached self (promised prom_src) mem_src)
         (EXCLUSIVE: forall loc' ts' (SELF: promised prom_src loc' ts') (OTHER: others loc' ts'), False)
     :
       exists prom_src' mem_src' self',
@@ -3369,269 +2811,6 @@ Section SIM.
         (<<PROMATTACH: promises_not_attached self' (promised prom_src') mem_src'>>)
   .
   Proof.
-    inv STEPTGT.
-
-    - hexploit add_succeed_wf; try apply MEM0. i. des.
-
-      assert (DISJOINTSRC:
-                forall to2 from2 msg2
-                       (GET2: Memory.get loc to2 mem_src = Some (from2, msg2)),
-                  Interval.disjoint (Time.middle from to, to) (from2, to2)).
-      { ii. specialize (MEM loc to2). inv MEM.
-        - rewrite GET2 in *. clarify.
-        - rewrite GET2 in *. clarify. eapply DISJOINT; eauto.
-          + instantiate (1:=x). inv LHS. econs; ss.
-            transitivity (Time.middle from to); auto.
-            eapply Time.middle_spec; auto.
-          + inv RHS. econs; ss. eapply TimeFacts.le_lt_lt; eauto.
-        - rewrite GET2 in *. clarify. eapply DISJOINT; eauto.
-          + instantiate (1:=x). inv LHS. econs; ss.
-            transitivity (Time.middle from to); auto.
-            eapply Time.middle_spec; auto.
-          + inv RHS. econs; ss. eapply TimeFacts.le_lt_lt; eauto. }
-      hexploit (@Memory.add_exists mem_src loc (Time.middle from to) to Message.reserve).
-      { auto. }
-      { eapply Time.middle_spec; auto. }
-      { econs. }
-      intros [mem_src' ADDMEM].
-      hexploit (@Memory.add_exists_le prom_src mem_src loc (Time.middle from to) to Message.reserve); eauto.
-      intros [prom_src' ADDPROM].
-      assert (PROMISESRC: Memory.promise prom_src mem_src loc (Time.middle from to) to Message.reserve prom_src' mem_src' Memory.op_kind_add).
-      { econs; eauto. i. clarify. }
-      assert (FUTURE: reserve_future_memory prom_src mem_src prom_src' mem_src').
-      { eauto. }
-
-      exists prom_src', mem_src',
-      (fun loc' ts' => if loc_ts_eq_dec (loc', ts') (loc, to)
-                       then msg_tgt <> Message.reserve else self loc' ts').
-      splits; auto.
-      + ii. erewrite (@Memory.add_o mem_src'); eauto.
-        erewrite (@Memory.add_o mem_tgt'); eauto.
-        des_ifs; try by (ss; des; clarify).
-        * ss. des; clarify. destruct msg_tgt.
-          { econs 3; eauto.
-            - right. clarify.
-            - left. eapply Time.middle_spec; eauto. }
-          { econs 2; eauto.
-            - ii. des; eauto. exfalso.
-              specialize (MEM loc to). eapply Memory.add_get0 in ADDMEM.
-              des. rewrite GET in *. inv MEM. eauto.
-            - left. eapply Time.middle_spec; eauto.
-            - i. clarify.
-          }
-      + ii. erewrite Memory.add_o in GET; eauto. des_ifs; eauto.
-        ss. des; clarify. exfalso.
-        specialize (MEM loc (Time.middle from to)). inv MEM.
-        { eapply NPROM; auto. }
-        { eapply NPROM; auto. }
-        { guardH PROM. exploit Memory.get_disjoint.
-          { eapply Memory.add_get1; try apply MEM0. symmetry. eapply H. }
-          { eapply Memory.add_get0; eauto. }
-          i. des.
-          - subst. eapply Time.lt_strorder.
-            instantiate (1:=to). rewrite <- x0 at 1.
-            eapply Time.middle_spec. auto.
-          - eapply x0.
-            + instantiate (1:=Time.middle from to). econs; ss.
-              * symmetry in H. eapply memory_get_ts_strong in H. des; auto.
-                subst. eapply TimeFacts.le_lt_lt.
-                { eapply Time.bot_spec. }
-                { eapply Time.middle_spec in TO1. des. eauto. }
-              * refl.
-            + econs; ss.
-              * eapply Time.middle_spec; eauto.
-              * left. eapply Time.middle_spec; eauto.
-        }
-      + ii. erewrite (@Memory.add_o prom_src'); eauto.
-        erewrite (@Memory.add_o prom_tgt'); eauto. des_ifs.
-        ss. des; clarify. destruct msg_tgt.
-        * econs 4; eauto. clarify.
-        * econs 3; eauto.
-      + ii. erewrite promised_add; eauto.
-        erewrite Memory.add_o in GET; eauto.
-        destruct msg_tgt; cycle 1.
-        { des_ifs; eauto; try by (ss; des; clarify). }
-        des_ifs; eauto; ss; des; clarify.
-        specialize (MEM loc ts1). rewrite GET in *. inv MEM.
-        { exfalso. destruct FROM.
-          { exploit DISJOINT.
-            - symmetry. eapply H.
-            - instantiate (1:=to). econs; ss. refl.
-            - econs; ss. apply memory_get_ts_le in GET; eauto.
-            - auto. }
-          { inv H0. exfalso. eapply ATTACH; eauto. }
-        }
-        { exfalso. destruct FROM.
-          { exploit DISJOINT.
-            - symmetry. eapply H.
-            - instantiate (1:=to). econs; ss. refl.
-            - econs; ss. apply memory_get_ts_le in GET; eauto.
-            - auto. }
-          { inv H0. exfalso. eapply ATTACH; eauto. }
-        }
-
-    - des. clarify.
-      exploit split_succeed_wf; try apply PROMISES. i. des.
-      dup GET2. apply WFTGT in GET0.
-      dup PROMISE. specialize (PROMISE0 loc ts3).
-      rewrite GET2 in PROMISE0.
-
-      assert (exists from_src, <<GETSRC: Memory.get loc ts3 prom_src = Some (from_src, Message.reserve)>>).
-      { inv PROMISE0; eauto. clarify. } des. rewrite GETSRC in *.
-
-      assert (EMPTY0: forall ts' (TS0: Time.lt from ts') (TS1: Time.lt ts' ts3),
-                 Memory.get loc ts' mem_tgt = None).
-      { i. destruct (Memory.get loc ts' mem_tgt) as [[from' msg']|] eqn:GET; auto.
-        exfalso. exploit Memory.get_disjoint.
-        { eapply GET. }
-        { eapply GET0. }
-        i. des; clarify.
-        - eapply Time.lt_strorder; eauto.
-        - eapply x0.
-          + instantiate (1:=ts'). econs; ss; [|refl].
-            apply memory_get_ts_strong in GET. des; clarify; auto.
-            exfalso. eapply Time.lt_strorder. eapply TimeFacts.lt_le_lt.
-            * eapply TS0.
-            * eapply Time.bot_spec.
-          + econs; ss. left. auto. }
-
-      assert (EMPTY1: forall to' msg' ts' (TS0: Time.lt from ts') (TS1: Time.lt ts' ts3)
-                             (GET: Memory.get loc to' mem_tgt = Some (ts', msg')),
-                 False).
-      { i. exploit Memory.get_disjoint.
-        { eapply GET. }
-        { eapply GET0. }
-        i. des; clarify.
-        - eapply Time.lt_strorder; eauto.
-        - hexploit memory_get_to_mon.
-          { eapply GET0. }
-          { eapply GET. }
-          { auto. } i.
-          eapply x0.
-          + instantiate (1:=ts3). econs; ss. left. auto.
-          + econs; ss; [|refl]. etrans; eauto. }
-
-      exploit (@promises_not_attached_replace_split self loc from_src (Time.middle from to) to ts3 prom_src mem_src); auto.
-      { i. specialize (PROMISE loc to0). rewrite GET in *. inv PROMISE; clarify. }
-      { eapply (@TimeFacts.le_lt_lt _ from); eauto. eapply Time.bot_spec. }
-      { eapply Time.middle_spec; eauto. }
-      { ii. inv H.
-        assert (exists from0' msg', <<GETTGT: Memory.get loc to0 mem_tgt = Some (from0', msg')>> /\ <<TS: Time.le from0' from0>>).
-        { dup MEM. specialize (MEM loc to0). rewrite GET in MEM. inv MEM; eauto. } des.
-        assert (TS1: Time.lt to0 ts3).
-        { eapply memory_get_to_mon; try apply GET; eauto.
-          inv ITV0. inv ITV. ss. eapply TimeFacts.lt_le_lt; eauto. }
-        erewrite EMPTY0 in GETTGT.
-        - clarify.
-        - inv ITV. inv ITV0. ss. eapply TimeFacts.lt_le_lt.
-          { eapply Time.middle_spec; eauto. }
-          { left. eapply TimeFacts.lt_le_lt; eauto. }
-        - auto.
-      }
-
-      intros [prom_src' [mem_src' ?]]. des.
-
-      assert (PROMISEDDIFF: promised prom_src' =
-                            fun loc' =>
-                              if (Loc.eq_dec loc' loc)
-                              then fun ts' => if (Time.eq_dec ts' to) then True else promised prom_src loc' ts'
-                              else promised prom_src loc').
-      { extensionality loc'. extensionality ts'.
-        apply Coq.Logic.PropExtensionality.propositional_extensionality.
-        split; i.
-        - inv H. erewrite PROMSPEC in GET. des_ifs; try by (ss; des; clarify).
-          + ss. des; clarify. econs; eauto.
-          + ss. des; clarify. econs; eauto.
-          + econs; eauto.
-        - specialize (PROMSPEC loc' ts'). des_ifs; try by (ss; des; clarify).
-          + econs; eauto.
-          + econs; eauto.
-          + inv H. erewrite <- PROMSPEC in *. econs; eauto.
-          + inv H. erewrite <- PROMSPEC in *. econs; eauto. }
-
-      exists prom_src', mem_src',
-      (fun loc' ts' => if loc_ts_eq_dec (loc', ts') (loc, to)
-                       then True else self loc' ts'). splits; auto.
-      + ii. erewrite MEMSPEC.
-        erewrite (@Memory.split_o mem_tgt'); eauto.
-        des_ifs; try by (ss; des; clarify).
-        * ss. des; clarify. econs 3; eauto.
-          { left. apply Time.middle_spec; eauto. }
-        * ss. des; clarify.
-          specialize (MEM loc ts3). rewrite GET0 in *.
-          apply WFSRC in GETSRC. rewrite GETSRC in *. inv MEM; eauto.
-          { econs 2; eauto. refl. }
-          { econs 3; eauto. refl. }
-      + ii. erewrite MEMSPEC in GET. des_ifs.
-        * ss. des; clarify. exfalso.
-          specialize (MEM loc (Time.middle from to)).
-          inv MEM; try by (exfalso; eauto). clear PROM. erewrite EMPTY0 in H.
-          { clarify. }
-          { eapply Time.middle_spec; eauto. }
-          { etrans; eauto. eapply Time.middle_spec; eauto. }
-        * ss. des; clarify. exfalso.
-          specialize (MEM loc from0).
-          inv MEM; try by (exfalso; eauto). clear PROM. erewrite EMPTY0 in H; auto.
-          { clarify. }
-        * eauto.
-      + ii. erewrite PROMSPEC.
-        erewrite (@Memory.split_o prom_tgt'); eauto. des_ifs.
-        * ss. des; clarify. econs; eauto.
-        * ss. des; clarify. inv PROMISE0; eauto.
-      + ii. erewrite MEMSPEC in GET. erewrite PROMISEDDIFF.
-        des_ifs; eauto; try by (ss; des; clarify).
-        * ss. des; clarify. econs; eauto.
-        * ss. des; clarify. exfalso.
-          exploit (@memory_get_from_inj mem_src' loc to ts1 ts3 msg Message.reserve).
-          { erewrite MEMSPEC. des_ifs; ss; des; clarify. }
-          { erewrite MEMSPEC. des_ifs; ss; des; clarify.
-            exfalso. eapply Time.lt_strorder; eauto. }
-          i. des; clarify.
-          { eapply Time.lt_strorder; eauto. }
-
-    - dup PROMISES. apply Memory.lower_get0 in PROMISES0. des. clarify.
-      dup GET. apply WFTGT in GET1.
-      dup PROMISE. specialize (PROMISE0 loc to). rewrite GET in *.
-      inv PROMISE0; clarify.
-      exists prom_src, mem_src, self. splits; auto.
-      + ii. erewrite (@Memory.lower_o mem_tgt'); eauto. des_ifs.
-        ss. des; clarify.
-        specialize (MEM loc to). rewrite GET1 in *. inv MSG_LE. inv MEM; eauto.
-        { exfalso. eapply NPROM. auto. }
-      + ii. eauto.
-      + ii. erewrite (@Memory.lower_o prom_tgt'); eauto. des_ifs.
-        ss. des; clarify. inv MSG_LE. rewrite <- H0. econs 4; eauto.
-
-    - hexploit Memory.remove_get0; try apply PROMISES. i. des.
-      dup GET. apply WFTGT in GET1.
-      dup PROMISE. specialize (PROMISE0 loc to). rewrite GET in *.
-      inv PROMISE0; clarify.
-
-      hexploit (@Memory.remove_exists prom_src loc from_src to Message.reserve).
-      { auto. }
-      intros [prom_src' REMOVEPROM].
-      hexploit (@Memory.remove_exists_le prom_src mem_src loc from_src to Message.reserve); eauto.
-      intros [mem_src' REMOVEMEM].
-      assert (PROMISESRC: Memory.promise prom_src mem_src loc from_src to Message.reserve prom_src' mem_src' Memory.op_kind_cancel).
-      { econs; eauto. }
-      assert (FUTURE: reserve_future_memory prom_src mem_src prom_src' mem_src').
-      { eauto. }
-
-      exists prom_src', mem_src',
-      (fun loc' ts' => if loc_ts_eq_dec (loc', ts') (loc, to)
-                       then False else self loc' ts').
-      splits; auto.
-      + ii. erewrite (@Memory.remove_o mem_src'); eauto.
-        erewrite (@Memory.remove_o mem_tgt'); eauto.
-        des_ifs; ss; des; clarify. econs. ii. des; clarify.
-        eapply EXCLUSIVE; eauto. econs; eauto.
-      + ii. erewrite Memory.remove_o in GET2; eauto. des_ifs. eauto.
-      + ii. erewrite (@Memory.remove_o prom_src'); eauto.
-        erewrite (@Memory.remove_o prom_tgt'); eauto. des_ifs.
-        ss. des; clarify. econs. ss.
-      + ii. erewrite Memory.remove_o in GET2; eauto.
-        erewrite promised_remove; eauto. des_ifs; eauto.
-        ss. des; clarify.
   Qed.
 
   Lemma sim_write_forget others self mem_src mem_tgt prom_src prom_tgt
@@ -3668,144 +2847,6 @@ Section SIM.
         (<<PROMATTACH: promises_not_attached self' (promised prom_src') mem_src'>>)
   .
   Proof.
-    dup STEPTGT. eapply Memory.remove_get0 in STEPTGT0. des.
-    dup PROMISE. specialize (PROMISE0 loc to). rewrite GET in PROMISE0.
-    inv PROMISE0; clarify. rename H0 into GETSRC. symmetry in GETSRC.
-    exploit promises_not_attached_replace_write; eauto.
-    { i. specialize (PROMISE loc to0). rewrite GET1 in *.
-      inv PROMISE; eauto. clarify. }
-    { eapply TimeFacts.le_lt_lt; eauto. eapply Time.bot_spec. }
-    { ii. inv H.
-      assert (exists from_tgt msg_tgt,
-                 (<<GETTGT0: Memory.get loc to0 mem_tgt = Some (from_tgt, msg_tgt)>>)).
-      { dup MEM. specialize (MEM0 loc to0).
-        rewrite GET1 in MEM0. inv MEM0; eauto. } des.
-      exploit Memory.get_disjoint.
-      { eapply GETTGT0. }
-      { eapply WFTGT. eapply GET. } i. des; clarify.
-      - dup GETSRC. apply WFSRC in GETSRC0. clarify.
-        inv ITV. inv ITV0. ss.
-        eapply Time.lt_strorder. eapply (@TimeFacts.lt_le_lt from0 ts); eauto.
-      - eapply x0.
-        + instantiate (1:=ts). econs; ss.
-          * inv ITV. inv ITV0. ss.
-            eapply TimeFacts.le_lt_lt; eauto.
-            specialize (MEM loc to0).
-            rewrite GET1 in *. rewrite GETTGT0 in *. inv MEM; ss.
-          * inv ITV0. ss.
-        + inv ITV; ss. econs; ss.
-          * eapply TimeFacts.le_lt_lt; eauto.
-          * etrans; eauto. eapply memory_get_ts_le; eauto. }
-
-    i. des.
-
-    exists (fun loc' ts' => if loc_ts_eq_dec (loc', ts') (loc, to)
-                            then False else self loc' ts'),
-    prom1, prom2, mem1, mem2, prom3, mem3. splits; eauto.
-    - ii. erewrite MEMSPEC. des_ifs.
-      + ss. des; clarify.
-        dup GET. eapply WFTGT in GET. rewrite GET. econs 2; eauto.
-        * ii. des; eauto.
-        * i. clarify.
-    - ii. erewrite MEMSPEC in GET1. des_ifs; eauto.
-      ss. des; clarify. exfalso.
-      dup MEM. specialize (MEM0 loc from0). inv MEM0; eauto.
-      clear PROM0. exploit Memory.get_disjoint.
-      { symmetry. eapply H. }
-      { apply WFTGT. apply GET. }
-      i. des; clarify.
-      { exfalso. eapply Time.lt_strorder; eauto. }
-      destruct FROM.
-      { exfalso. eapply x0.
-        - instantiate (1:=from0). econs; ss.
-          + symmetry in H. apply memory_get_ts_strong in H. des; auto.
-            clarify. exfalso. eapply Time.lt_strorder.
-            eapply (@TimeFacts.le_lt_lt Time.bot from); eauto.
-            eapply Time.bot_spec.
-          + refl.
-        - econs; ss. left. auto. }
-      { inv H1. exploit ATTACHED; eauto. i. inv x. rewrite GET1 in *. clarify. }
-    - ii. erewrite PROMSPEC. erewrite (@Memory.remove_o prom_tgt'); eauto. des_ifs.
-      + ss. des; clarify. econs; eauto.
-    - ii. erewrite MEMSPEC in GET1. des_ifs.
-      + ss. des; clarify. exfalso.
-        dup MEM. specialize (MEM0 loc ts0). inv MEM0; eauto.
-        clear PROM0. exploit Memory.get_disjoint.
-        { symmetry. eapply H. }
-        { apply WFTGT. apply GET. }
-        i. des; clarify.
-        destruct FROM.
-        { exfalso. eapply x0.
-          - instantiate (1:=ts0). econs; ss.
-            + symmetry in H. apply memory_get_ts_strong in H. des; auto.
-              clarify. exfalso. eapply Time.lt_strorder.
-              eapply (@TimeFacts.le_lt_lt Time.bot from); eauto.
-              eapply Time.bot_spec.
-            + refl.
-          - econs; ss. left. auto. }
-        { inv H1. exploit ATTACHED; eauto. i. inv x. rewrite GET1 in *. clarify. }
-      + exploit PROMATTACH; eauto. i. inv x.
-        specialize (PROMSPEC loc0 ts1). des_ifs.
-        * ss. des; clarify.
-        * erewrite <- PROMSPEC in *. econs; eauto.
-  Qed.
-
-  Lemma reserve_future_memory_steps
-        lang st vw sc prom0 mem0 prom1 mem1
-        (FUTURE: reserve_future_memory prom0 mem0 prom1 mem1)
-    :
-      exists tr,
-        (<<STEPS: Trace.steps tr
-                              (Thread.mk lang st (Local.mk vw prom0) sc mem0)
-                              (Thread.mk lang st (Local.mk vw prom1) sc mem1)>>).
-  Proof.
-    ginduction FUTURE; eauto. i. exploit IHFUTURE; eauto. i. des.
-    esplits. eapply Trace.steps_trans; [|apply STEPS|ss].
-    econs 1. econs; eauto.
-  Qed.
-
-  Lemma reserve_future_memory_unchangable
-        prom0 mem0 prom1 mem1 loc to from msg
-        (FUTURE: reserve_future_memory prom0 mem0 prom1 mem1)
-        (UNCH: unchangable mem0 prom0 loc to from msg)
-    :
-      unchangable mem1 prom1 loc to from msg.
-  Proof.
-    ginduction FUTURE; eauto. i. exploit IHFUTURE; eauto.
-    eapply unchangable_promise; eauto.
-  Qed.
-
-  Lemma reserve_future_memory_future
-        vw sc prom0 mem0 prom1 mem1
-        (LOCAL: Local.wf (Local.mk vw prom0) mem0)
-        (SC: Memory.closed_timemap sc mem0)
-        (MEM: Memory.closed mem0)
-        (FUTURE: reserve_future_memory prom0 mem0 prom1 mem1)
-    :
-      (<<LOCAL: Local.wf (Local.mk vw prom1) mem1>>) /\
-      (<<SC: Memory.closed_timemap sc mem1>>) /\
-      (<<MEM: Memory.closed mem1>>).
-  Proof.
-    ginduction FUTURE; eauto. i.
-    exploit Local.promise_step_future.
-    { econs.
-      - instantiate (9:=Local.mk vw prom0). eauto.
-      - eauto.
-      - eauto. }
-    all: eauto. i. des. ss. eapply IHFUTURE; eauto.
-  Qed.
-
-  Lemma reserve_future_concrete_same_promise2 prom0 mem0 prom1 mem1 loc from to val released
-        (FUTURE: reserve_future_memory prom0 mem0 prom1 mem1)
-        (GET: Memory.get loc to prom1 = Some (from, Message.concrete val released))
-    :
-      Memory.get loc to prom0 = Some (from, Message.concrete val released).
-  Proof.
-    ginduction FUTURE; auto. i. apply IHFUTURE in GET; auto.
-    inv HD; des; clarify.
-    - erewrite Memory.add_o in GET; eauto. des_ifs.
-    - erewrite Memory.lower_o in GET; eauto. des_ifs.
-    - erewrite Memory.remove_o in GET; eauto. des_ifs.
   Qed.
 
   Lemma sim_write_step_forget
@@ -3908,31 +2949,6 @@ Section SIM.
       eapply reserve_future_concrete_same_promise2 in GET; eauto.
       specialize (PROMISE0 loc t). rewrite GET in PROMISE0. inv PROMISE0; ss. }
     { etrans; eauto. }
-  Qed.
-
-  Lemma reserve_future_read_commute
-        vw0 prom0 mem0 loc to val released ord vw1 prom' prom1 mem1
-        (READ: Local.read_step (Local.mk vw0 prom0) mem0 loc to val released ord (Local.mk vw1 prom'))
-        (FUTURE: reserve_future_memory prom0 mem0 prom1 mem1)
-    :
-      Local.read_step (Local.mk vw0 prom1) mem1 loc to val released ord (Local.mk vw1 prom1).
-  Proof.
-    inv READ. clarify. econs; eauto.
-    eapply reserve_future_concrete_same; eauto.
-  Qed.
-
-  Lemma joined_view_semi_closed
-        views view mem loc ts
-        (MEM: List.Forall (fun vw => semi_closed_view vw mem loc ts) views)
-        (JOINED: joined_view views view)
-        (INHABITED: Memory.inhabited mem)
-    :
-      semi_closed_view view mem loc ts.
-  Proof.
-    ginduction JOINED; eauto.
-    - i. eapply closed_view_semi_closed. apply Memory.closed_view_bot. auto.
-    - i. eapply semi_closed_view_join; eauto.
-      eapply List.Forall_forall in VIEW; [|eauto]. ss.
   Qed.
 
   Lemma sim_thread_step' others self lang st lc_src lc_tgt sc mem_src mem_tgt pf e_tgt
@@ -4093,30 +3109,6 @@ Section SIM.
         * refl.
   Qed.
 
-  Lemma traces_steps_future
-        lang tr e1 e2
-        (STEPS: @Trace.steps lang tr e1 e2)
-        (WF1: Local.wf e1.(Thread.local) e1.(Thread.memory))
-        (SC1: Memory.closed_timemap e1.(Thread.sc) e1.(Thread.memory))
-        (CLOSED1: Memory.closed e1.(Thread.memory)):
-    (<<WF2: Local.wf e2.(Thread.local) e2.(Thread.memory)>>) /\
-    (<<SC2: Memory.closed_timemap e2.(Thread.sc) e2.(Thread.memory)>>) /\
-    (<<CLOSED2: Memory.closed e2.(Thread.memory)>>) /\
-    (<<TVIEW_FUTURE: TView.le e1.(Thread.local).(Local.tview) e2.(Thread.local).(Local.tview)>>) /\
-    (<<SC_FUTURE: TimeMap.le e1.(Thread.sc) e2.(Thread.sc)>>) /\
-    (<<MEM_FUTURE: Memory.future e1.(Thread.memory) e2.(Thread.memory)>>)
-  .
-  Proof.
-    ginduction STEPS.
-    - i. splits; auto.
-      + refl.
-      + refl.
-    - i. exploit Thread.step_future; eauto. i. des.
-      exploit IHSTEPS; eauto. i. des. splits; auto.
-      + etrans; eauto.
-      + etrans; eauto.
-      + etrans; eauto.
-  Qed.
 
   Lemma sim_thread_step others self lang st lc_src lc_tgt sc mem_src mem_tgt pf e_tgt
         st' lc_tgt' sc' mem_tgt' views views'
